<?xml version="1.0" encoding="UTF-8"?>
<!DOCTYPE rdf:RDF [
	<!ENTITY dct "http://purl.org/dc/terms/">
	<!ENTITY fibo-fbc-dae-dbt "https://spec.edmcouncil.org/fibo/ontology/FBC/DebtAndEquities/Debt/">
	<!ENTITY fibo-fbc-fi-fi "https://spec.edmcouncil.org/fibo/ontology/FBC/FinancialInstruments/FinancialInstruments/">
	<!ENTITY fibo-fnd-acc-aeq "https://spec.edmcouncil.org/fibo/ontology/FND/Accounting/AccountingEquity/">
	<!ENTITY fibo-fnd-agr-ctr "https://spec.edmcouncil.org/fibo/ontology/FND/Agreements/Contracts/">
	<!ENTITY fibo-fnd-arr-arr "https://spec.edmcouncil.org/fibo/ontology/FND/Arrangements/Arrangements/">
	<!ENTITY fibo-fnd-rel-rel "https://spec.edmcouncil.org/fibo/ontology/FND/Relations/Relations/">
	<!ENTITY fibo-fnd-utl-av "https://spec.edmcouncil.org/fibo/ontology/FND/Utilities/AnnotationVocabulary/">
	<!ENTITY fibo-sec-dbt-ab-pbs "https://spec.edmcouncil.org/fibo/ontology/SEC/Debt/AssetBackedSecurities/PoolBackedSecurities/">
	<!ENTITY fibo-sec-dbt-bnd "https://spec.edmcouncil.org/fibo/ontology/SEC/Debt/Bonds/">
	<!ENTITY fibo-sec-dbt-dbti "https://spec.edmcouncil.org/fibo/ontology/SEC/Debt/DebtInstruments/">
	<!ENTITY fibo-sec-sec-iss "https://spec.edmcouncil.org/fibo/ontology/SEC/Securities/SecuritiesIssuance/">
	<!ENTITY fibo-sec-sec-pls "https://spec.edmcouncil.org/fibo/ontology/SEC/Securities/Pools/">
	<!ENTITY owl "http://www.w3.org/2002/07/owl#">
	<!ENTITY rdf "http://www.w3.org/1999/02/22-rdf-syntax-ns#">
	<!ENTITY rdfs "http://www.w3.org/2000/01/rdf-schema#">
	<!ENTITY skos "http://www.w3.org/2004/02/skos/core#">
	<!ENTITY sm "http://www.omg.org/techprocess/ab/SpecificationMetadata/">
	<!ENTITY xsd "http://www.w3.org/2001/XMLSchema#">
]>
<rdf:RDF xml:base="https://spec.edmcouncil.org/fibo/ontology/SEC/Debt/AssetBackedSecurities/PoolBackedSecurities/"
	xmlns:dct="http://purl.org/dc/terms/"
	xmlns:fibo-fbc-dae-dbt="https://spec.edmcouncil.org/fibo/ontology/FBC/DebtAndEquities/Debt/"
	xmlns:fibo-fbc-fi-fi="https://spec.edmcouncil.org/fibo/ontology/FBC/FinancialInstruments/FinancialInstruments/"
	xmlns:fibo-fnd-acc-aeq="https://spec.edmcouncil.org/fibo/ontology/FND/Accounting/AccountingEquity/"
	xmlns:fibo-fnd-agr-ctr="https://spec.edmcouncil.org/fibo/ontology/FND/Agreements/Contracts/"
	xmlns:fibo-fnd-arr-arr="https://spec.edmcouncil.org/fibo/ontology/FND/Arrangements/Arrangements/"
	xmlns:fibo-fnd-rel-rel="https://spec.edmcouncil.org/fibo/ontology/FND/Relations/Relations/"
	xmlns:fibo-fnd-utl-av="https://spec.edmcouncil.org/fibo/ontology/FND/Utilities/AnnotationVocabulary/"
	xmlns:fibo-sec-dbt-ab-pbs="https://spec.edmcouncil.org/fibo/ontology/SEC/Debt/AssetBackedSecurities/PoolBackedSecurities/"
	xmlns:fibo-sec-dbt-bnd="https://spec.edmcouncil.org/fibo/ontology/SEC/Debt/Bonds/"
	xmlns:fibo-sec-dbt-dbti="https://spec.edmcouncil.org/fibo/ontology/SEC/Debt/DebtInstruments/"
	xmlns:fibo-sec-sec-iss="https://spec.edmcouncil.org/fibo/ontology/SEC/Securities/SecuritiesIssuance/"
	xmlns:fibo-sec-sec-pls="https://spec.edmcouncil.org/fibo/ontology/SEC/Securities/Pools/"
	xmlns:owl="http://www.w3.org/2002/07/owl#"
	xmlns:rdf="http://www.w3.org/1999/02/22-rdf-syntax-ns#"
	xmlns:rdfs="http://www.w3.org/2000/01/rdf-schema#"
	xmlns:skos="http://www.w3.org/2004/02/skos/core#"
	xmlns:sm="http://www.omg.org/techprocess/ab/SpecificationMetadata/"
	xmlns:xsd="http://www.w3.org/2001/XMLSchema#">
	
	<owl:Ontology rdf:about="https://spec.edmcouncil.org/fibo/ontology/SEC/Debt/AssetBackedSecurities/PoolBackedSecurities/">
		<rdfs:label xml:lang="en">Pool-backed Securities Ontology</rdfs:label>
		<dct:abstract>Concepts common to asset backed and mortgage backed securities, including pools, instruments, prospectuses and deals common concepts. 
		Note that in common industry parlance, the term &apos;asset backed security&apos; is used to refer to securities which specifically do not have a mortgage loan pool as their underlying asset. For this reason, this ontology provides a common parent to both asset backed and mortgage backed securities, which is effectively an asset backed security in the broader sense. This has been labeled as &apos;pool backed security instrument&apos; as there is no common industry name for this common parent class, other than &apos;asset backed security&apos;.</dct:abstract>
		<dct:license rdf:datatype="&xsd;anyURI">http://opensource.org/licenses/MIT</dct:license>
		<sm:contentLanguage rdf:datatype="&xsd;anyURI">https://www.w3.org/TR/owl2-quick-reference/</sm:contentLanguage>
		<sm:copyright>Copyright (c) 2015-2021 EDM Council, Inc.</sm:copyright>
		<sm:dependsOn rdf:datatype="&xsd;anyURI">https://spec.edmcouncil.org/fibo/ontology/FBC/</sm:dependsOn>
		<sm:dependsOn rdf:datatype="&xsd;anyURI">https://spec.edmcouncil.org/fibo/ontology/FND/</sm:dependsOn>
		<sm:dependsOn rdf:datatype="&xsd;anyURI">https://spec.edmcouncil.org/fibo/ontology/SEC/Debt/Bonds/</sm:dependsOn>
		<sm:dependsOn rdf:datatype="&xsd;anyURI">https://spec.edmcouncil.org/fibo/ontology/SEC/Debt/DebtInstruments/</sm:dependsOn>
		<sm:dependsOn rdf:datatype="&xsd;anyURI">https://spec.edmcouncil.org/fibo/ontology/SEC/Securities/Pools/</sm:dependsOn>
		<sm:dependsOn rdf:datatype="&xsd;anyURI">https://spec.edmcouncil.org/fibo/ontology/SEC/Securities/SecuritiesIssuance/</sm:dependsOn>
		<sm:fileAbbreviation>fibo-sec-dbt-ab-pbs</sm:fileAbbreviation>
		<sm:filename>PoolBackedSecurities.rdf</sm:filename>
		<owl:imports rdf:resource="https://spec.edmcouncil.org/fibo/ontology/FBC/DebtAndEquities/Debt/"/>
		<owl:imports rdf:resource="https://spec.edmcouncil.org/fibo/ontology/FBC/FinancialInstruments/FinancialInstruments/"/>
		<owl:imports rdf:resource="https://spec.edmcouncil.org/fibo/ontology/FND/Accounting/AccountingEquity/"/>
		<owl:imports rdf:resource="https://spec.edmcouncil.org/fibo/ontology/FND/Agreements/Contracts/"/>
		<owl:imports rdf:resource="https://spec.edmcouncil.org/fibo/ontology/FND/Arrangements/Arrangements/"/>
		<owl:imports rdf:resource="https://spec.edmcouncil.org/fibo/ontology/FND/Relations/Relations/"/>
		<owl:imports rdf:resource="https://spec.edmcouncil.org/fibo/ontology/FND/Utilities/AnnotationVocabulary/"/>
		<owl:imports rdf:resource="https://spec.edmcouncil.org/fibo/ontology/SEC/Debt/Bonds/"/>
		<owl:imports rdf:resource="https://spec.edmcouncil.org/fibo/ontology/SEC/Debt/DebtInstruments/"/>
		<owl:imports rdf:resource="https://spec.edmcouncil.org/fibo/ontology/SEC/Securities/Pools/"/>
		<owl:imports rdf:resource="https://spec.edmcouncil.org/fibo/ontology/SEC/Securities/SecuritiesIssuance/"/>
		<owl:versionIRI rdf:resource="https://spec.edmcouncil.org/fibo/ontology/SEC/Debt/AssetBackedSecurities/PoolBackedSecurities/"/>
		<fibo-fnd-utl-av:hasMaturityLevel rdf:resource="&fibo-fnd-utl-av;Provisional"/>
	</owl:Ontology>
	
	<owl:Class rdf:about="&fibo-sec-dbt-ab-pbs;CashStructuredFinanceInstrument">
		<rdfs:subClassOf rdf:resource="&fibo-sec-dbt-ab-pbs;StructuredFinanceInstrument"/>
		<rdfs:subClassOf>
			<owl:Restriction>
				<owl:onProperty rdf:resource="&fibo-sec-dbt-ab-pbs;isTrancheOf"/>
				<owl:someValuesFrom rdf:resource="&fibo-sec-dbt-ab-pbs;SecuritizedDebtPool"/>
			</owl:Restriction>
		</rdfs:subClassOf>
		<rdfs:label xml:lang="en">cash-structured finance instrument</rdfs:label>
		<skos:definition xml:lang="en">A structured finance instrument with a real asset underlying.</skos:definition>
	</owl:Class>
	
	<owl:Class rdf:about="&fibo-sec-dbt-ab-pbs;CashStructuredFinanceInstrumentPool">
		<rdfs:subClassOf rdf:resource="&fibo-sec-dbt-ab-pbs;StructuredFinanceInstrumentPool"/>
		<rdfs:label xml:lang="en">cash-structured finance instrument pool</rdfs:label>
		<skos:definition xml:lang="en">A pool investment consisting of a collection of cash structured finance instruments.</skos:definition>
	</owl:Class>
	
	<owl:Class rdf:about="&fibo-sec-dbt-ab-pbs;CollateralizedDebt">
		<rdfs:subClassOf rdf:resource="&fibo-sec-dbt-dbti;PubliclyIssuedDebt"/>
		<rdfs:subClassOf>
			<owl:Restriction>
				<owl:onProperty rdf:resource="&fibo-fbc-dae-dbt;isCollateralizedBy"/>
				<owl:someValuesFrom rdf:resource="&fibo-fnd-acc-aeq;FinancialAsset"/>
			</owl:Restriction>
		</rdfs:subClassOf>
		<rdfs:label xml:lang="en">collateralized debt</rdfs:label>
		<skos:definition xml:lang="en">Debt issued under some Security, with some Collateral.</skos:definition>
	</owl:Class>
	
	<owl:Class rdf:about="&fibo-sec-dbt-ab-pbs;CollateralizedObligationOffering">
		<rdfs:subClassOf rdf:resource="&fibo-sec-dbt-dbti;DebtOffering"/>
		<rdfs:label xml:lang="en">collateralized obligation</rdfs:label>
		<skos:definition xml:lang="en">Pending further investigation. At present: CDO = issued against pool of securities MBS = issued against pool of individual debts (base loans) Action: identify if this is the case. Option 1: Model as it was; Option 2: Add a level of detail in between, whereby there is a pool of pools or some other such thing Option 3: this is a terminological thing only in that CDOs are never referred to as a parent of CMO for purely teerminological reasons as per ABS v MBS in which case we would add in a terminological layer.</skos:definition>
	</owl:Class>
	
	<owl:Class rdf:about="&fibo-sec-dbt-ab-pbs;PoolBackedDealProspectus">
		<rdfs:subClassOf rdf:resource="&fibo-sec-sec-iss;Prospectus"/>
		<rdfs:label xml:lang="en">pool backed deal prospectus</rdfs:label>
		<skos:definition xml:lang="en">Prospectus describing the terms of the issue and each of the instruments included in the pool backed security issue. Term origin:SMER</skos:definition>
	</owl:Class>
	
	<owl:Class rdf:about="&fibo-sec-dbt-ab-pbs;PoolBackedSecuritiesOffering">
		<rdfs:subClassOf rdf:resource="&fibo-sec-dbt-dbti;DebtOffering"/>
		<rdfs:subClassOf>
			<owl:Restriction>
				<owl:onProperty rdf:resource="&fibo-fnd-rel-rel;appliesTo"/>
				<owl:someValuesFrom rdf:resource="&fibo-sec-dbt-ab-pbs;PoolBackedSecurity"/>
			</owl:Restriction>
		</rdfs:subClassOf>
		<rdfs:subClassOf>
			<owl:Restriction>
				<owl:onProperty rdf:resource="&fibo-fnd-rel-rel;refersTo"/>
				<owl:someValuesFrom rdf:resource="&fibo-sec-dbt-ab-pbs;SecuritizedDebtPool"/>
			</owl:Restriction>
		</rdfs:subClassOf>
		<rdfs:label xml:lang="en">pool-backed securities offering</rdfs:label>
		<skos:definition xml:lang="en">The issue of a series of Pool Backed Security certificates. These are (at least in this context) securities issued backed by a pool of individual loans, mortgages or other individual loan products.</skos:definition>
		<skos:editorialNote xml:lang="en">This term makes the distinction, perhaps artificial, between deals backed by pools of individual debt (this term), and deals backed by pools of securities (collateralized deals). This structure of relations between kinds of deals may prove to be a little artificial, but it reflects the structure of relations between kinds of securities, arrived at in earlier SME reviews. That is, Pool Backed Security (which breaks down into ABS and MBS) has a pool of individual loan products (a sub type of which is mortgage loans). The terms reflect the fact that in common parlance the term &quot;ABS&quot; is taken to mean something which is explicitly NOT a MBS but can be any other type of loan or credit based security, hence the creation of the non standard term &quot;Pool Backed Security&quot;. The naming of deals simply attempts to reflect that. Terms to be included in Deal (per PoC conversations): Underwriters Issuer Deal Number Series number Deal Value Different collateral pools that support the deal. Review existing terms and make sure all covered.</skos:editorialNote>
	</owl:Class>
	
	<owl:Class rdf:about="&fibo-sec-dbt-ab-pbs;PoolBackedSecurity">
		<rdfs:subClassOf rdf:resource="&fibo-sec-dbt-ab-pbs;StructuredFinanceInstrument"/>
		<rdfs:subClassOf>
			<owl:Restriction>
				<owl:onProperty rdf:resource="&fibo-fnd-agr-ctr;definesTermsFor"/>
				<owl:someValuesFrom rdf:resource="&fibo-sec-dbt-ab-pbs;CollateralizedDebt"/>
			</owl:Restriction>
		</rdfs:subClassOf>
		<rdfs:subClassOf>
			<owl:Restriction>
				<owl:onProperty rdf:resource="&fibo-sec-dbt-ab-pbs;isTrancheOf"/>
				<owl:someValuesFrom rdf:resource="&fibo-sec-sec-pls;DebtPool"/>
			</owl:Restriction>
		</rdfs:subClassOf>
		<rdfs:label xml:lang="en">pool-backed security</rdfs:label>
		<skos:definition xml:lang="en">bond or note that derives its cashflow from some underlying pool of debt in which loans or mortgage advanced to borrowers are pooled together for the purposes of creating this type of security</skos:definition>
	</owl:Class>
	
	<owl:Class rdf:about="&fibo-sec-dbt-ab-pbs;SecuritizedDebtPool">
		<rdfs:subClassOf rdf:resource="&fibo-sec-sec-pls;DebtPool"/>
		<rdfs:label xml:lang="en">securitized debt pool</rdfs:label>
		<skos:definition xml:lang="en">pool of individual debt instruments (such as loans or mortgages) that is securitized as part of the issue of some security</skos:definition>
	</owl:Class>
	
	<owl:Class rdf:about="&fibo-sec-dbt-ab-pbs;StructuredFinanceInstrument">
		<rdfs:subClassOf rdf:resource="&fibo-sec-dbt-dbti;TradableDebtInstrument"/>
		<rdfs:label xml:lang="en">structured finance instrument</rdfs:label>
		<skos:definition xml:lang="en">debt instrument that has periodic principal payments with the amount of principal that is paid being dictated by a published factor</skos:definition>
		<skos:example xml:lang="en">Collateralized debt obligations (CDOs), synthetic financial instruments, collateralized bond obligations (CBOs), and syndicated loans are examples of structured finance instruments.</skos:example>
		<fibo-fnd-utl-av:explanatoryNote xml:lang="en">This may be either an invented product (synthetic) or based on a real underlying asset pool. Either way, the underlying is defined by the issuing bank or investment company. These are traded. This is based on tranches of underlying asset pools. These are defined by the issuing bank or investment company.</fibo-fnd-utl-av:explanatoryNote>
	</owl:Class>
	
	<owl:Class rdf:about="&fibo-sec-dbt-ab-pbs;StructuredFinanceInstrumentPool">
		<rdfs:subClassOf rdf:resource="&fibo-sec-sec-pls;InstrumentPool"/>
		<rdfs:subClassOf>
			<owl:Restriction>
				<owl:onProperty rdf:resource="&fibo-fnd-arr-arr;hasConstituent"/>
				<owl:someValuesFrom rdf:resource="&fibo-sec-dbt-ab-pbs;StructuredFinanceInstrument"/>
			</owl:Restriction>
		</rdfs:subClassOf>
		<rdfs:label xml:lang="en">structured finance instrument pool</rdfs:label>
		<skos:definition xml:lang="en">pool consisting of a collection of structured finance instruments</skos:definition>
	</owl:Class>
	
	<owl:ObjectProperty rdf:about="&fibo-sec-dbt-ab-pbs;backs">
		<rdfs:label xml:lang="en">backs</rdfs:label>
		<rdfs:domain rdf:resource="&fibo-sec-dbt-ab-pbs;SecuritizedDebtPool"/>
		<rdfs:range rdf:resource="&fibo-sec-dbt-ab-pbs;CashStructuredFinanceInstrument"/>
		<owl:inverseOf rdf:resource="&fibo-sec-dbt-ab-pbs;isTrancheOf"/>
	</owl:ObjectProperty>
	
	<owl:ObjectProperty rdf:about="&fibo-sec-dbt-ab-pbs;isTrancheOf">
		<rdfs:label xml:lang="en">is tranche of</rdfs:label>
		<rdfs:domain rdf:resource="&fibo-sec-dbt-ab-pbs;CashStructuredFinanceInstrument"/>
		<rdfs:range rdf:resource="&fibo-sec-dbt-ab-pbs;SecuritizedDebtPool"/>
		<skos:definition xml:lang="en">The asset pool which is the underlying of a traditional or cash structured finance instrument. This is a real pool of real assets, as distinct from synthetic pools.</skos:definition>
	</owl:ObjectProperty>
	
	<owl:DatatypeProperty rdf:about="&fibo-sec-dbt-ab-pbs;passThrough">
		<rdfs:label xml:lang="en">pass through</rdfs:label>
		<rdfs:domain rdf:resource="&fibo-sec-dbt-ab-pbs;CashStructuredFinanceInstrument"/>
		<rdfs:range rdf:resource="&xsd;boolean"/>
		<skos:definition xml:lang="en">Whether the cash flows from the underlying asset pool are passed through to the investor by way of redemption payments.</skos:definition>
	</owl:DatatypeProperty>
	
	<owl:Class rdf:about="&fibo-sec-sec-pls;DebtPool">
		<rdfs:subClassOf>
			<owl:Restriction>
				<owl:onProperty rdf:resource="&fibo-sec-dbt-ab-pbs;backs"/>
				<owl:someValuesFrom rdf:resource="&fibo-sec-dbt-ab-pbs;PoolBackedSecurity"/>
			</owl:Restriction>
		</rdfs:subClassOf>
	</owl:Class>

</rdf:RDF>