<?xml version="1.0" encoding="UTF-8"?>
<!DOCTYPE rdf:RDF [
	<!ENTITY dct "http://purl.org/dc/terms/">
	<!ENTITY fibo-be-fct-pub "https://spec.edmcouncil.org/fibo/ontology/BE/FunctionalEntities/Publishers/">
	<!ENTITY fibo-be-le-lp "https://spec.edmcouncil.org/fibo/ontology/BE/LegalEntities/LegalPersons/">
	<!ENTITY fibo-der-com-ctr "https://spec.edmcouncil.org/fibo/ontology/DER/CommoditiesDerivatives/CommoditiesContracts/">
	<!ENTITY fibo-der-der-opt "https://spec.edmcouncil.org/fibo/ontology/DER/DerivativesContracts/Options/">
	<!ENTITY fibo-der-drc-bsc "https://spec.edmcouncil.org/fibo/ontology/DER/DerivativesContracts/DerivativesBasics/">
	<!ENTITY fibo-der-drc-fwd "https://spec.edmcouncil.org/fibo/ontology/DER/DerivativesContracts/Forwards/">
	<!ENTITY fibo-der-drc-swp "https://spec.edmcouncil.org/fibo/ontology/DER/DerivativesContracts/Swaps/">
	<!ENTITY fibo-der-fx-ctr "https://spec.edmcouncil.org/fibo/ontology/DER/FxDerivatives/FxContracts/">
	<!ENTITY fibo-der-sbd-sbd "https://spec.edmcouncil.org/fibo/ontology/DER/SecurityBasedDerivatives/SecurityBasedDerivatives/">
	<!ENTITY fibo-fbc-dae-gty "https://spec.edmcouncil.org/fibo/ontology/FBC/DebtAndEquities/Guaranty/">
	<!ENTITY fibo-fbc-fct-mkt "https://spec.edmcouncil.org/fibo/ontology/FBC/FunctionalEntities/Markets/">
	<!ENTITY fibo-fbc-fct-ra "https://spec.edmcouncil.org/fibo/ontology/FBC/FunctionalEntities/RegistrationAuthorities/">
	<!ENTITY fibo-fbc-fi-fi "https://spec.edmcouncil.org/fibo/ontology/FBC/FinancialInstruments/FinancialInstruments/">
	<!ENTITY fibo-fbc-fi-ip "https://spec.edmcouncil.org/fibo/ontology/FBC/FinancialInstruments/InstrumentPricing/">
	<!ENTITY fibo-fbc-pas-caa "https://spec.edmcouncil.org/fibo/ontology/FBC/ProductsAndServices/ClientsAndAccounts/">
	<!ENTITY fibo-fbc-pas-fpas "https://spec.edmcouncil.org/fibo/ontology/FBC/ProductsAndServices/FinancialProductsAndServices/">
	<!ENTITY fibo-fnd-acc-cur "https://spec.edmcouncil.org/fibo/ontology/FND/Accounting/CurrencyAmount/">
	<!ENTITY fibo-fnd-agr-ctr "https://spec.edmcouncil.org/fibo/ontology/FND/Agreements/Contracts/">
	<!ENTITY fibo-fnd-arr-arr "https://spec.edmcouncil.org/fibo/ontology/FND/Arrangements/Arrangements/">
	<!ENTITY fibo-fnd-dt-fd "https://spec.edmcouncil.org/fibo/ontology/FND/DatesAndTimes/FinancialDates/">
	<!ENTITY fibo-fnd-dt-oc "https://spec.edmcouncil.org/fibo/ontology/FND/DatesAndTimes/Occurrences/">
	<!ENTITY fibo-fnd-gao-obj "https://spec.edmcouncil.org/fibo/ontology/FND/GoalsAndObjectives/Objectives/">
	<!ENTITY fibo-fnd-law-lcap "https://spec.edmcouncil.org/fibo/ontology/FND/Law/LegalCapacity/">
	<!ENTITY fibo-fnd-oac-own "https://spec.edmcouncil.org/fibo/ontology/FND/OwnershipAndControl/Ownership/">
	<!ENTITY fibo-fnd-pas-pas "https://spec.edmcouncil.org/fibo/ontology/FND/ProductsAndServices/ProductsAndServices/">
	<!ENTITY fibo-fnd-pty-pty "https://spec.edmcouncil.org/fibo/ontology/FND/Parties/Parties/">
	<!ENTITY fibo-fnd-pty-rl "https://spec.edmcouncil.org/fibo/ontology/FND/Parties/Roles/">
	<!ENTITY fibo-fnd-qt-qtu "https://spec.edmcouncil.org/fibo/ontology/FND/Quantities/QuantitiesAndUnits/">
	<!ENTITY fibo-fnd-rel-rel "https://spec.edmcouncil.org/fibo/ontology/FND/Relations/Relations/">
	<!ENTITY fibo-fnd-utl-alx "https://spec.edmcouncil.org/fibo/ontology/FND/Utilities/Analytics/">
	<!ENTITY fibo-fnd-utl-av "https://spec.edmcouncil.org/fibo/ontology/FND/Utilities/AnnotationVocabulary/">
	<!ENTITY fibo-ind-fx-fx "https://spec.edmcouncil.org/fibo/ontology/IND/ForeignExchange/ForeignExchange/">
	<!ENTITY fibo-ind-ind-ind "https://spec.edmcouncil.org/fibo/ontology/IND/Indicators/Indicators/">
	<!ENTITY fibo-ind-mkt-bas "https://spec.edmcouncil.org/fibo/ontology/IND/MarketIndices/BasketIndices/">
	<!ENTITY fibo-sec-dbt-bnd "https://spec.edmcouncil.org/fibo/ontology/SEC/Debt/Bonds/">
	<!ENTITY fibo-sec-dbt-ex "https://spec.edmcouncil.org/fibo/ontology/SEC/Debt/ExerciseConventions/">
	<!ENTITY fibo-sec-eq-eq "https://spec.edmcouncil.org/fibo/ontology/SEC/Equities/EquityInstruments/">
	<!ENTITY fibo-sec-sec-lst "https://spec.edmcouncil.org/fibo/ontology/SEC/Securities/SecuritiesListings/">
	<!ENTITY owl "http://www.w3.org/2002/07/owl#">
	<!ENTITY rdf "http://www.w3.org/1999/02/22-rdf-syntax-ns#">
	<!ENTITY rdfs "http://www.w3.org/2000/01/rdf-schema#">
	<!ENTITY skos "http://www.w3.org/2004/02/skos/core#">
	<!ENTITY sm "http://www.omg.org/techprocess/ab/SpecificationMetadata/">
	<!ENTITY xsd "http://www.w3.org/2001/XMLSchema#">
]>
<rdf:RDF xml:base="https://spec.edmcouncil.org/fibo/ontology/DER/DerivativesContracts/Options/"
	xmlns:dct="http://purl.org/dc/terms/"
	xmlns:fibo-be-fct-pub="https://spec.edmcouncil.org/fibo/ontology/BE/FunctionalEntities/Publishers/"
	xmlns:fibo-be-le-lp="https://spec.edmcouncil.org/fibo/ontology/BE/LegalEntities/LegalPersons/"
	xmlns:fibo-der-com-ctr="https://spec.edmcouncil.org/fibo/ontology/DER/CommoditiesDerivatives/CommoditiesContracts/"
	xmlns:fibo-der-der-opt="https://spec.edmcouncil.org/fibo/ontology/DER/DerivativesContracts/Options/"
	xmlns:fibo-der-drc-bsc="https://spec.edmcouncil.org/fibo/ontology/DER/DerivativesContracts/DerivativesBasics/"
	xmlns:fibo-der-drc-fwd="https://spec.edmcouncil.org/fibo/ontology/DER/DerivativesContracts/Forwards/"
	xmlns:fibo-der-drc-swp="https://spec.edmcouncil.org/fibo/ontology/DER/DerivativesContracts/Swaps/"
	xmlns:fibo-der-fx-ctr="https://spec.edmcouncil.org/fibo/ontology/DER/FxDerivatives/FxContracts/"
	xmlns:fibo-der-sbd-sbd="https://spec.edmcouncil.org/fibo/ontology/DER/SecurityBasedDerivatives/SecurityBasedDerivatives/"
	xmlns:fibo-fbc-dae-gty="https://spec.edmcouncil.org/fibo/ontology/FBC/DebtAndEquities/Guaranty/"
	xmlns:fibo-fbc-fct-mkt="https://spec.edmcouncil.org/fibo/ontology/FBC/FunctionalEntities/Markets/"
	xmlns:fibo-fbc-fct-ra="https://spec.edmcouncil.org/fibo/ontology/FBC/FunctionalEntities/RegistrationAuthorities/"
	xmlns:fibo-fbc-fi-fi="https://spec.edmcouncil.org/fibo/ontology/FBC/FinancialInstruments/FinancialInstruments/"
	xmlns:fibo-fbc-fi-ip="https://spec.edmcouncil.org/fibo/ontology/FBC/FinancialInstruments/InstrumentPricing/"
	xmlns:fibo-fbc-pas-caa="https://spec.edmcouncil.org/fibo/ontology/FBC/ProductsAndServices/ClientsAndAccounts/"
	xmlns:fibo-fbc-pas-fpas="https://spec.edmcouncil.org/fibo/ontology/FBC/ProductsAndServices/FinancialProductsAndServices/"
	xmlns:fibo-fnd-acc-cur="https://spec.edmcouncil.org/fibo/ontology/FND/Accounting/CurrencyAmount/"
	xmlns:fibo-fnd-agr-ctr="https://spec.edmcouncil.org/fibo/ontology/FND/Agreements/Contracts/"
	xmlns:fibo-fnd-arr-arr="https://spec.edmcouncil.org/fibo/ontology/FND/Arrangements/Arrangements/"
	xmlns:fibo-fnd-dt-fd="https://spec.edmcouncil.org/fibo/ontology/FND/DatesAndTimes/FinancialDates/"
	xmlns:fibo-fnd-dt-oc="https://spec.edmcouncil.org/fibo/ontology/FND/DatesAndTimes/Occurrences/"
	xmlns:fibo-fnd-gao-obj="https://spec.edmcouncil.org/fibo/ontology/FND/GoalsAndObjectives/Objectives/"
	xmlns:fibo-fnd-law-lcap="https://spec.edmcouncil.org/fibo/ontology/FND/Law/LegalCapacity/"
	xmlns:fibo-fnd-oac-own="https://spec.edmcouncil.org/fibo/ontology/FND/OwnershipAndControl/Ownership/"
	xmlns:fibo-fnd-pas-pas="https://spec.edmcouncil.org/fibo/ontology/FND/ProductsAndServices/ProductsAndServices/"
	xmlns:fibo-fnd-pty-pty="https://spec.edmcouncil.org/fibo/ontology/FND/Parties/Parties/"
	xmlns:fibo-fnd-pty-rl="https://spec.edmcouncil.org/fibo/ontology/FND/Parties/Roles/"
	xmlns:fibo-fnd-qt-qtu="https://spec.edmcouncil.org/fibo/ontology/FND/Quantities/QuantitiesAndUnits/"
	xmlns:fibo-fnd-rel-rel="https://spec.edmcouncil.org/fibo/ontology/FND/Relations/Relations/"
	xmlns:fibo-fnd-utl-alx="https://spec.edmcouncil.org/fibo/ontology/FND/Utilities/Analytics/"
	xmlns:fibo-fnd-utl-av="https://spec.edmcouncil.org/fibo/ontology/FND/Utilities/AnnotationVocabulary/"
	xmlns:fibo-ind-fx-fx="https://spec.edmcouncil.org/fibo/ontology/IND/ForeignExchange/ForeignExchange/"
	xmlns:fibo-ind-ind-ind="https://spec.edmcouncil.org/fibo/ontology/IND/Indicators/Indicators/"
	xmlns:fibo-ind-mkt-bas="https://spec.edmcouncil.org/fibo/ontology/IND/MarketIndices/BasketIndices/"
	xmlns:fibo-sec-dbt-bnd="https://spec.edmcouncil.org/fibo/ontology/SEC/Debt/Bonds/"
	xmlns:fibo-sec-dbt-ex="https://spec.edmcouncil.org/fibo/ontology/SEC/Debt/ExerciseConventions/"
	xmlns:fibo-sec-eq-eq="https://spec.edmcouncil.org/fibo/ontology/SEC/Equities/EquityInstruments/"
	xmlns:fibo-sec-sec-lst="https://spec.edmcouncil.org/fibo/ontology/SEC/Securities/SecuritiesListings/"
	xmlns:owl="http://www.w3.org/2002/07/owl#"
	xmlns:rdf="http://www.w3.org/1999/02/22-rdf-syntax-ns#"
	xmlns:rdfs="http://www.w3.org/2000/01/rdf-schema#"
	xmlns:skos="http://www.w3.org/2004/02/skos/core#"
	xmlns:sm="http://www.omg.org/techprocess/ab/SpecificationMetadata/"
	xmlns:xsd="http://www.w3.org/2001/XMLSchema#">
	
	<owl:Ontology rdf:about="https://spec.edmcouncil.org/fibo/ontology/DER/DerivativesContracts/Options/">
		<rdfs:label xml:lang="en">Options Ontology</rdfs:label>
		<dct:abstract>Concepts common to all option contracts and their corresponding transactions. An option gives one party (the holder) the right to purchase or sell the underlying commodity at a given time or times in the future (as determined by the exercise convention), if they choose to do so. Includes option features, these being definitions of how the option comes into or ceases being in force when a given event occurs along with a range of other variations.</dct:abstract>
		<dct:license rdf:datatype="&xsd;anyURI">http://opensource.org/licenses/MIT</dct:license>
		<sm:contentLanguage rdf:datatype="&xsd;anyURI">https://www.w3.org/TR/owl2-quick-reference/</sm:contentLanguage>
		<sm:copyright>Copyright (c) 2015-2021 EDM Council, Inc.</sm:copyright>
		<sm:dependsOn rdf:resource="https://spec.edmcouncil.org/fibo/ontology/BE/"/>
		<sm:dependsOn rdf:resource="https://spec.edmcouncil.org/fibo/ontology/FBC/"/>
		<sm:dependsOn rdf:resource="https://spec.edmcouncil.org/fibo/ontology/FND/"/>
		<sm:dependsOn rdf:resource="https://spec.edmcouncil.org/fibo/ontology/IND/"/>
		<sm:dependsOn rdf:resource="https://spec.edmcouncil.org/fibo/ontology/SEC/"/>
		<sm:fileAbbreviation>fibo-der-der-opt</sm:fileAbbreviation>
		<sm:filename>Options.rdf</sm:filename>
		<owl:imports rdf:resource="https://spec.edmcouncil.org/fibo/ontology/BE/FunctionalEntities/Publishers/"/>
		<owl:imports rdf:resource="https://spec.edmcouncil.org/fibo/ontology/BE/LegalEntities/LegalPersons/"/>
		<owl:imports rdf:resource="https://spec.edmcouncil.org/fibo/ontology/DER/CommoditiesDerivatives/CommoditiesContracts/"/>
		<owl:imports rdf:resource="https://spec.edmcouncil.org/fibo/ontology/DER/DerivativesContracts/DerivativesBasics/"/>
		<owl:imports rdf:resource="https://spec.edmcouncil.org/fibo/ontology/DER/DerivativesContracts/Forwards/"/>
		<owl:imports rdf:resource="https://spec.edmcouncil.org/fibo/ontology/DER/DerivativesContracts/Swaps/"/>
		<owl:imports rdf:resource="https://spec.edmcouncil.org/fibo/ontology/DER/FxDerivatives/FxContracts/"/>
		<owl:imports rdf:resource="https://spec.edmcouncil.org/fibo/ontology/DER/SecurityBasedDerivatives/SecurityBasedDerivatives/"/>
		<owl:imports rdf:resource="https://spec.edmcouncil.org/fibo/ontology/FBC/DebtAndEquities/Guaranty/"/>
		<owl:imports rdf:resource="https://spec.edmcouncil.org/fibo/ontology/FBC/FinancialInstruments/FinancialInstruments/"/>
		<owl:imports rdf:resource="https://spec.edmcouncil.org/fibo/ontology/FBC/FinancialInstruments/InstrumentPricing/"/>
		<owl:imports rdf:resource="https://spec.edmcouncil.org/fibo/ontology/FBC/FunctionalEntities/Markets/"/>
		<owl:imports rdf:resource="https://spec.edmcouncil.org/fibo/ontology/FBC/FunctionalEntities/RegistrationAuthorities/"/>
		<owl:imports rdf:resource="https://spec.edmcouncil.org/fibo/ontology/FBC/ProductsAndServices/ClientsAndAccounts/"/>
		<owl:imports rdf:resource="https://spec.edmcouncil.org/fibo/ontology/FBC/ProductsAndServices/FinancialProductsAndServices/"/>
		<owl:imports rdf:resource="https://spec.edmcouncil.org/fibo/ontology/FND/Accounting/CurrencyAmount/"/>
		<owl:imports rdf:resource="https://spec.edmcouncil.org/fibo/ontology/FND/Agreements/Contracts/"/>
		<owl:imports rdf:resource="https://spec.edmcouncil.org/fibo/ontology/FND/Arrangements/Arrangements/"/>
		<owl:imports rdf:resource="https://spec.edmcouncil.org/fibo/ontology/FND/DatesAndTimes/FinancialDates/"/>
		<owl:imports rdf:resource="https://spec.edmcouncil.org/fibo/ontology/FND/DatesAndTimes/Occurrences/"/>
		<owl:imports rdf:resource="https://spec.edmcouncil.org/fibo/ontology/FND/GoalsAndObjectives/Objectives/"/>
		<owl:imports rdf:resource="https://spec.edmcouncil.org/fibo/ontology/FND/Law/LegalCapacity/"/>
		<owl:imports rdf:resource="https://spec.edmcouncil.org/fibo/ontology/FND/OwnershipAndControl/Ownership/"/>
		<owl:imports rdf:resource="https://spec.edmcouncil.org/fibo/ontology/FND/Parties/Parties/"/>
		<owl:imports rdf:resource="https://spec.edmcouncil.org/fibo/ontology/FND/Parties/Roles/"/>
		<owl:imports rdf:resource="https://spec.edmcouncil.org/fibo/ontology/FND/ProductsAndServices/ProductsAndServices/"/>
		<owl:imports rdf:resource="https://spec.edmcouncil.org/fibo/ontology/FND/Quantities/QuantitiesAndUnits/"/>
		<owl:imports rdf:resource="https://spec.edmcouncil.org/fibo/ontology/FND/Relations/Relations/"/>
		<owl:imports rdf:resource="https://spec.edmcouncil.org/fibo/ontology/FND/Utilities/Analytics/"/>
		<owl:imports rdf:resource="https://spec.edmcouncil.org/fibo/ontology/FND/Utilities/AnnotationVocabulary/"/>
		<owl:imports rdf:resource="https://spec.edmcouncil.org/fibo/ontology/IND/ForeignExchange/ForeignExchange/"/>
		<owl:imports rdf:resource="https://spec.edmcouncil.org/fibo/ontology/IND/Indicators/Indicators/"/>
		<owl:imports rdf:resource="https://spec.edmcouncil.org/fibo/ontology/IND/MarketIndices/BasketIndices/"/>
		<owl:imports rdf:resource="https://spec.edmcouncil.org/fibo/ontology/SEC/Debt/Bonds/"/>
		<owl:imports rdf:resource="https://spec.edmcouncil.org/fibo/ontology/SEC/Debt/ExerciseConventions/"/>
		<owl:imports rdf:resource="https://spec.edmcouncil.org/fibo/ontology/SEC/Equities/EquityInstruments/"/>
		<owl:imports rdf:resource="https://spec.edmcouncil.org/fibo/ontology/SEC/Securities/SecuritiesListings/"/>
		<owl:versionIRI rdf:resource="https://spec.edmcouncil.org/fibo/ontology/DER/DerivativesContracts/Options/"/>
		<fibo-fnd-utl-av:hasMaturityLevel rdf:resource="&fibo-fnd-utl-av;Provisional"/>
	</owl:Ontology>
	
	<owl:Class rdf:about="&fibo-der-drc-bsc;DerivativesClearingOrganization">
		<fibo-fnd-utl-av:explanatoryNote xml:lang="en">For options, the derivatives clearing organization is responsible for clearing transactions for put and call options on common stocks and other equity issues, stock indexes, foreign currencies, interest rate composites and single-stock futures. e.g. Options Clearing Corporation (US). In Canada the equivalent is In the US, the Options Clearing Corporation defines defaults e.g. lot sizes. This applies to equity options, index options, flex options, yield based options and short dated options. It does not apply to other types of option. Its roles are: 1. Clearing 2. Advocate for sound business practice. Similar to regulator though not officially one. Has a role in risk management Full list from OCC website: OCC clears transactions for put and call options on common stocks and other equity issues, stock indexes, foreign currencies, interest rate composites and single-stock futures</fibo-fnd-utl-av:explanatoryNote>
	</owl:Class>
	
	<owl:Class rdf:about="&fibo-der-der-opt;AsianExerciseTerms">
		<rdfs:subClassOf rdf:resource="&fibo-sec-dbt-ex;ExerciseTerms"/>
		<rdfs:subClassOf>
			<owl:Restriction>
				<owl:onProperty rdf:resource="&fibo-sec-dbt-ex;hasExerciseDate"/>
				<owl:onClass rdf:resource="&fibo-fnd-dt-fd;ExplicitDate"/>
				<owl:qualifiedCardinality rdf:datatype="&xsd;nonNegativeInteger">1</owl:qualifiedCardinality>
			</owl:Restriction>
		</rdfs:subClassOf>
		<rdfs:label xml:lang="en">Asian exercise terms</rdfs:label>
		<skos:definition xml:lang="en">exercise terms whereby the payoff is determined by the average underlying price over some pre-set period of time</skos:definition>
		<fibo-fnd-utl-av:explanatoryNote xml:lang="en">Because of the averaging feature, Asian options reduce the volatility inherent in the option; therefore, Asian options are typically cheaper than European or American options.</fibo-fnd-utl-av:explanatoryNote>
	</owl:Class>
	
	<owl:Class rdf:about="&fibo-der-der-opt;AssetMaximumOrMinimumPayoutCommitment">
		<rdfs:subClassOf rdf:resource="&fibo-der-der-opt;ConditionalPayoutCommitment"/>
		<rdfs:label xml:lang="en">asset maximum or minimum payout commitment</rdfs:label>
		<skos:definition xml:lang="en">A commitment to pay out on the maximum or minimum of a set of assets. Further Notes Maximum of n Assets This rainbow is similar to the best of n assets plus cash we referred to in part a, with the exception that no cash payoff is possible and there is a strike price for this type of option. The payoff of a call and put are given as: Rainbow-Call = max[0, max(S1, S2) - X] Rainbow-Put = max[0, X - max(S1, S2)] Minimum of n Assets The counterpart to a maximum of n assets, this rainbow pays out the value of the underperformer of the n assets. The payoff for minimum of 2 asset rainbow calls and puts are given as: Rainbow-Call = max[0, mainS1, S2) - X] Rainbow-Put = max[0, X - min(S1, S2)]</skos:definition>
	</owl:Class>
	
	<owl:Class rdf:about="&fibo-der-der-opt;AssetOrNothingPayoutCommitment">
		<rdfs:subClassOf rdf:resource="&fibo-der-der-opt;BinaryPayoutCommitment"/>
		<rdfs:label xml:lang="en">asset or nothing payout commitment</rdfs:label>
		<owl:disjointWith rdf:resource="&fibo-der-der-opt;CashOrNothingPayoutCommitment"/>
	</owl:Class>
	
	<owl:Class rdf:about="&fibo-der-der-opt;BestOfAssetsPlusCashPayoutCommitment">
		<rdfs:subClassOf rdf:resource="&fibo-der-der-opt;ConditionalPayoutCommitment"/>
		<rdfs:subClassOf>
			<owl:Restriction>
				<owl:onProperty rdf:resource="&fibo-fbc-fct-ra;specifies"/>
				<owl:someValuesFrom rdf:resource="&fibo-der-der-opt;PayoffAssetsList"/>
			</owl:Restriction>
		</rdfs:subClassOf>
		<rdfs:label xml:lang="en">best of assets plus cash payout commitment</rdfs:label>
		<skos:definition xml:lang="en">A commitment to pay out on the best of a number of assets, plus cash.</skos:definition>
		<fibo-fnd-utl-av:explanatoryNote xml:lang="en">This type of rainbow effectively has n + 1 payoff possibilities. If we consider a 2 asset &quot;best of plus cash&quot;, the payoff at expiry is a choice between Asset 1, Asset 2, or the predetermined cash amount. There is no strike price and the payoff is given as: Rainbow = max(S1, S2, Cash;T)</fibo-fnd-utl-av:explanatoryNote>
	</owl:Class>
	
	<owl:Class rdf:about="&fibo-der-der-opt;BetterOrWorseOfAssetsPayoutCommitment">
		<rdfs:subClassOf rdf:resource="&fibo-der-der-opt;ConditionalPayoutCommitment"/>
		<rdfs:subClassOf>
			<owl:Restriction>
				<owl:onProperty rdf:resource="&fibo-der-der-opt;references"/>
				<owl:someValuesFrom rdf:resource="&fibo-der-der-opt;PayoffAssetsList"/>
			</owl:Restriction>
		</rdfs:subClassOf>
		<rdfs:label xml:lang="en">better or worse of assets payout commitment</rdfs:label>
		<skos:definition xml:lang="en">A commitment to pay out on the best or worst of a number of assets.</skos:definition>
		<fibo-fnd-utl-av:explanatoryNote xml:lang="en">Better of n Assets This type of rainbow is similar to the best of n assets plus cash but with the exception that there is no possible cash payoff, and X is set to 0. With this in mind, a better of 2 assets rainbow is essentially a two-asset call option, with a payoff being: Rainbow = max[0, max(S1, S2)] Worse of n Assets Essentially the opposite to the better of n assets, with the payoff being on the asset with the lower value. We can give the payoff for this option on 2 assets as: Rainbow = max[0, min(S1, S2)]</fibo-fnd-utl-av:explanatoryNote>
	</owl:Class>
	
	<owl:Class rdf:about="&fibo-der-der-opt;BinaryPayoutCommitment">
		<rdfs:subClassOf rdf:resource="&fibo-der-der-opt;OptionPayoutCommitment"/>
		<rdfs:label xml:lang="en">binary payout commitment</rdfs:label>
		<owl:disjointWith rdf:resource="&fibo-der-der-opt;ConditionalPayoutCommitment"/>
	</owl:Class>
	
	<owl:Class rdf:about="&fibo-der-der-opt;BondOption">
		<rdfs:subClassOf rdf:resource="&fibo-der-der-opt;OptionOnFuture"/>
		<rdfs:subClassOf rdf:resource="&fibo-der-sbd-sbd;DebtInstrumentDerivative"/>
		<rdfs:subClassOf>
			<owl:Restriction>
				<owl:onProperty rdf:resource="&fibo-der-drc-bsc;hasUnderlier"/>
				<owl:someValuesFrom rdf:resource="&fibo-sec-dbt-bnd;Bond"/>
			</owl:Restriction>
		</rdfs:subClassOf>
		<rdfs:label xml:lang="en">bond option</rdfs:label>
		<skos:definition xml:lang="en">option on a futures contract whose underlying asset is a bond</skos:definition>
		<fibo-fnd-utl-av:explanatoryNote xml:lang="en">When exercised, the holder exercises the right to buy the future on a Bond, s/he does not exercise the right to buy a bond. For example an option on a Treasury Bill is an option on a T Bill Future, not on a T Bill itself. Hence these are defined as a kind of futures option.</fibo-fnd-utl-av:explanatoryNote>
	</owl:Class>
	
	<owl:Class rdf:about="&fibo-der-der-opt;CalculatedPayoutCommitment">
		<rdfs:subClassOf rdf:resource="&fibo-der-der-opt;OptionPayoutCommitment"/>
		<rdfs:label xml:lang="en">calculated payout commitment</rdfs:label>
		<owl:disjointWith rdf:resource="&fibo-der-der-opt;ConditionalPayoutCommitment"/>
		<owl:disjointWith rdf:resource="&fibo-der-der-opt;LinearPayoutCommitment"/>
	</owl:Class>
	
	<owl:Class rdf:about="&fibo-der-der-opt;CallOption">
		<rdfs:subClassOf rdf:resource="&fibo-fbc-fi-fi;Option"/>
		<rdfs:subClassOf>
			<owl:Restriction>
				<owl:onProperty rdf:resource="&fibo-fnd-pas-pas;hasBuyer"/>
				<owl:someValuesFrom>
					<owl:Class>
						<owl:unionOf rdf:parseType="Collection">
							<rdf:Description rdf:about="&fibo-der-der-opt;OptionHolder">
							</rdf:Description>
							<rdf:Description rdf:about="&fibo-der-drc-bsc;PayingParty">
							</rdf:Description>
						</owl:unionOf>
					</owl:Class>
				</owl:someValuesFrom>
			</owl:Restriction>
		</rdfs:subClassOf>
		<rdfs:subClassOf>
			<owl:Restriction>
				<owl:onProperty rdf:resource="&fibo-fnd-pas-pas;hasSeller"/>
				<owl:someValuesFrom>
					<owl:Class>
						<owl:unionOf rdf:parseType="Collection">
							<rdf:Description rdf:about="&fibo-der-der-opt;OptionIssuer">
							</rdf:Description>
							<rdf:Description rdf:about="&fibo-der-drc-bsc;ReceivingParty">
							</rdf:Description>
						</owl:unionOf>
					</owl:Class>
				</owl:someValuesFrom>
			</owl:Restriction>
		</rdfs:subClassOf>
		<rdfs:label xml:lang="en">call option</rdfs:label>
		<skos:definition xml:lang="en">option giving the buyer (holder) the right, but not the obligation, to buy the assets specified at a fixed price or formula, on or before a specified date. The seller of the call option assumes the obligation of delivering the assets specified should the buyer exercise his option.</skos:definition>
		<fibo-fnd-utl-av:adaptedFrom xml:lang="en">ISO 10962, Securities and related financial instruments - Classification of financial instruments (CFI) code, Fourth Edition, 2019.</fibo-fnd-utl-av:adaptedFrom>
		<fibo-fnd-utl-av:explanatoryNote xml:lang="en">The seller (issuer) of the call option assumes the obligation of delivering the assets specified should the buyer exercise his option. The buyer has the option, but not the obligation, to purchase the underlying asset.</fibo-fnd-utl-av:explanatoryNote>
	</owl:Class>
	
	<owl:Class rdf:about="&fibo-der-der-opt;CashOrNothingPayoutCommitment">
		<rdfs:subClassOf rdf:resource="&fibo-der-der-opt;BinaryPayoutCommitment"/>
		<rdfs:label xml:lang="en">cash or nothing payout commitment</rdfs:label>
		<skos:definition xml:lang="en">A commitment to pay out on a binary option, as cash or nothing.</skos:definition>
	</owl:Class>
	
	<owl:Class rdf:about="&fibo-der-der-opt;ChooserOption">
		<rdfs:subClassOf rdf:resource="&fibo-fbc-fi-fi;Option"/>
		<rdfs:subClassOf>
			<owl:Restriction>
				<owl:onProperty rdf:resource="&fibo-der-der-opt;hasOptionTypeElectionDate"/>
				<owl:someValuesFrom rdf:resource="&fibo-fnd-dt-fd;ExplicitDate"/>
			</owl:Restriction>
		</rdfs:subClassOf>
		<rdfs:subClassOf>
			<owl:Restriction>
				<owl:onProperty rdf:resource="&fibo-fnd-rel-rel;refersTo"/>
				<owl:someValuesFrom>
					<owl:Class>
						<owl:unionOf rdf:parseType="Collection">
							<rdf:Description rdf:about="&fibo-der-der-opt;CallOption">
							</rdf:Description>
							<rdf:Description rdf:about="&fibo-der-der-opt;PutOption">
							</rdf:Description>
						</owl:unionOf>
					</owl:Class>
				</owl:someValuesFrom>
			</owl:Restriction>
		</rdfs:subClassOf>
		<rdfs:label xml:lang="en">chooser option</rdfs:label>
		<skos:definition xml:lang="en">exotic option that is transacted in the present, but that at some specified future date is chosen to be either a put or a call option</skos:definition>
		<fibo-fnd-utl-av:adaptedFrom xml:lang="en">Commodity Futures Trading Commission (CFTC) glossary, https://www.cftc.gov/LearnAndProtect/EducationCenter/CFTCGlossary/glossary_c.html</fibo-fnd-utl-av:adaptedFrom>
	</owl:Class>
	
	<owl:Class rdf:about="&fibo-der-der-opt;CommodityOption">
		<rdfs:subClassOf rdf:resource="&fibo-der-com-ctr;CommodityDerivative"/>
		<rdfs:subClassOf rdf:resource="&fibo-der-der-opt;OptionOnFuture"/>
		<rdfs:subClassOf>
			<owl:Restriction>
				<owl:onProperty rdf:resource="&fibo-der-drc-bsc;hasUnderlier"/>
				<owl:someValuesFrom rdf:resource="&fibo-der-com-ctr;CommodityFuture"/>
			</owl:Restriction>
		</rdfs:subClassOf>
		<rdfs:label xml:lang="en">commodity option</rdfs:label>
		<skos:definition xml:lang="en">option giving buyer (holder) the right, but not the obligation, to buy or sell a futures contract for a stated commodity at a given strike price on or before the exercise date</skos:definition>
	</owl:Class>
	
	<owl:Class rdf:about="&fibo-der-der-opt;ConditionalPayoutCommitment">
		<rdfs:subClassOf rdf:resource="&fibo-der-der-opt;OptionPayoutCommitment"/>
		<rdfs:label xml:lang="en">conditional payout commitment</rdfs:label>
		<owl:disjointWith rdf:resource="&fibo-der-der-opt;LinearPayoutCommitment"/>
	</owl:Class>
	
	<owl:Class rdf:about="&fibo-der-der-opt;CurrencyOptionExerciseTerms">
		<rdfs:subClassOf rdf:resource="&fibo-sec-dbt-ex;ExerciseTerms"/>
		<rdfs:subClassOf>
			<owl:Restriction>
				<owl:onProperty rdf:resource="&fibo-der-der-opt;delivery"/>
				<owl:someValuesFrom rdf:resource="&fibo-fnd-acc-cur;AmountOfMoney"/>
			</owl:Restriction>
		</rdfs:subClassOf>
		<rdfs:label xml:lang="en">currency option exercise terms</rdfs:label>
		<skos:definition xml:lang="en">Contractual terms defining when or under what circumstances an currency option is to be exercised.</skos:definition>
		<fibo-fnd-utl-av:explanatoryNote xml:lang="en">Also includes terms defining delivery when the contract is exercised. Delivery for currency options is by way of cash.</fibo-fnd-utl-av:explanatoryNote>
	</owl:Class>
	
	<owl:Class rdf:about="&fibo-der-der-opt;DefinedConditionsPayoutCommitment">
		<rdfs:subClassOf rdf:resource="&fibo-der-der-opt;OptionPayoutCommitment"/>
		<rdfs:label xml:lang="en">defined conditions payout commitment</rdfs:label>
		<skos:definition xml:lang="en">A commitment which is only made when certain defined conditions are met. Further notes: Like all contractual commitments, the details of the commitment (and in this case, the conditions) are defined in the corresponding Contractual Terms. These set out what the commitment is and what the conditions are under which it is to be met. Term introduced in order to support digital and other exotic options. Note this is similar to but distinct from commitments where the specific nature of the commitment (typically a cashflow) is defined by resolving some mathematical formula i.e. where the commitment to do something is not conditional but the precise monetary amounts (payment, settlement) are.</skos:definition>
	</owl:Class>
	
	<owl:Class rdf:about="&fibo-der-der-opt;EquityIndexOptionUnderlying">
		<rdfs:subClassOf rdf:resource="&fibo-der-drc-bsc;Underlier"/>
		<rdfs:subClassOf>
			<owl:Restriction>
				<owl:onProperty rdf:resource="&fibo-fnd-rel-rel;hasIdentity"/>
				<owl:someValuesFrom rdf:resource="&fibo-ind-mkt-bas;EquityIndex"/>
			</owl:Restriction>
		</rdfs:subClassOf>
		<rdfs:label xml:lang="en">equity index option underlying</rdfs:label>
		<skos:definition xml:lang="en">The inderlying of the equity index option, which is a reference index consisting of shares.</skos:definition>
		<skos:editorialNote xml:lang="en">Review session note 16 Dec 2009: Nature of the &quot;Underlying&quot; as a class here: Somebody takes a defined Pf of those at that time. Modeling response: this describes a different sort of equity option, one based on a locally defined basket of equities. This has not been modeled. An equity index as defined here and in the Indices and Indicators part of the model is a published figure, out out by an index publisher. The composition of the basiet underkying that index is a matter for the publisher and not for the Options Contract. It sounds as though a locally defined basket may be used as another kind of Underlying, and may be loosely referred to as an index option, however that&apos;s not the term modeled here.</skos:editorialNote>
	</owl:Class>
	
	<owl:Class rdf:about="&fibo-der-der-opt;EquityOption">
		<rdfs:subClassOf rdf:resource="&fibo-der-sbd-sbd;EquityDerivative"/>
		<rdfs:subClassOf rdf:resource="&fibo-fbc-fi-fi;Option"/>
		<rdfs:subClassOf>
			<owl:Restriction>
				<owl:onProperty rdf:resource="&fibo-der-drc-bsc;hasUnderlier"/>
				<owl:someValuesFrom rdf:resource="&fibo-der-sbd-sbd;EquityObservable"/>
			</owl:Restriction>
		</rdfs:subClassOf>
		<rdfs:subClassOf>
			<owl:Restriction>
				<owl:onProperty rdf:resource="&fibo-sec-dbt-ex;hasExerciseTerms"/>
				<owl:someValuesFrom rdf:resource="&fibo-der-der-opt;StockOptionExerciseTerms"/>
			</owl:Restriction>
		</rdfs:subClassOf>
		<rdfs:label xml:lang="en">equity option</rdfs:label>
		<skos:definition xml:lang="en">Equity options are the most common type of equity derivative. They provide the right, but not the obligation to trade a quantity of stock at a set price at a future time.</skos:definition>
	</owl:Class>
	
	<owl:Class rdf:about="&fibo-der-der-opt;ExchangeTradedEquityIndexOption">
		<rdfs:subClassOf rdf:resource="&fibo-der-der-opt;ExchangeTradedOption"/>
		<rdfs:subClassOf rdf:resource="&fibo-der-sbd-sbd;EquityDerivative"/>
		<rdfs:subClassOf>
			<owl:Restriction>
				<owl:onProperty rdf:resource="&fibo-der-drc-bsc;hasUnderlier"/>
				<owl:someValuesFrom rdf:resource="&fibo-der-der-opt;EquityIndexOptionUnderlying"/>
			</owl:Restriction>
		</rdfs:subClassOf>
		<rdfs:subClassOf>
			<owl:Restriction>
				<owl:onProperty rdf:resource="&fibo-sec-dbt-ex;hasExerciseTerms"/>
				<owl:someValuesFrom rdf:resource="&fibo-der-der-opt;IndexOptionExerciseTerms"/>
			</owl:Restriction>
		</rdfs:subClassOf>
		<rdfs:label xml:lang="en">exchange traded equity index option</rdfs:label>
		<skos:definition xml:lang="en">Equity Index options offer the investor an opportunity to either capitalize on an expected market move or to protect holdings in the underlying instruments. The difference is that the underlying instruments are indexes.</skos:definition>
		<fibo-fnd-utl-av:explanatoryNote xml:lang="en">These indexes can reflect the characteristics of either the broad equity market as a whole or specific industry sectors within the marketplace.</fibo-fnd-utl-av:explanatoryNote>
	</owl:Class>
	
	<owl:Class rdf:about="&fibo-der-der-opt;ExchangeTradedOption">
		<rdfs:subClassOf rdf:resource="&fibo-fbc-fi-fi;Option"/>
		<rdfs:subClassOf>
			<owl:Restriction>
				<owl:onProperty rdf:resource="&fibo-fnd-agr-ctr;hasContractualElement"/>
				<owl:onClass rdf:resource="&fibo-der-der-opt;OptionBarrierFeatureTerms"/>
				<owl:maxQualifiedCardinality rdf:datatype="&xsd;nonNegativeInteger">2</owl:maxQualifiedCardinality>
			</owl:Restriction>
		</rdfs:subClassOf>
		<rdfs:subClassOf>
			<owl:Restriction>
				<owl:onProperty rdf:resource="&fibo-der-drc-fwd;hasContractSize"/>
				<owl:someValuesFrom rdf:resource="&xsd;integer"/>
			</owl:Restriction>
		</rdfs:subClassOf>
		<rdfs:subClassOf>
			<owl:Restriction>
				<owl:onProperty rdf:resource="&fibo-fbc-dae-gty;hasGuarantor"/>
				<owl:someValuesFrom rdf:resource="&fibo-der-der-opt;OptionGuarantor"/>
			</owl:Restriction>
		</rdfs:subClassOf>
		<rdfs:subClassOf>
			<owl:Restriction>
				<owl:onProperty rdf:resource="&fibo-fbc-fi-ip;hasPriceDeterminationMethod"/>
				<owl:someValuesFrom rdf:resource="&fibo-fbc-fi-ip;PriceDeterminationMethod"/>
			</owl:Restriction>
		</rdfs:subClassOf>
		<rdfs:subClassOf>
			<owl:Restriction>
				<owl:onProperty rdf:resource="&fibo-fnd-agr-ctr;hasContractDuration"/>
				<owl:someValuesFrom rdf:resource="&fibo-fnd-dt-fd;ExplicitDuration"/>
			</owl:Restriction>
		</rdfs:subClassOf>
		<rdfs:subClassOf>
			<owl:Restriction>
				<owl:onProperty rdf:resource="&fibo-fnd-agr-ctr;hasCounterparty"/>
				<owl:someValuesFrom rdf:resource="&fibo-der-der-opt;TradedOptionsCounterparty"/>
			</owl:Restriction>
		</rdfs:subClassOf>
		<rdfs:subClassOf>
			<owl:Restriction>
				<owl:onProperty rdf:resource="&fibo-fnd-pas-pas;hasSeller"/>
				<owl:someValuesFrom>
					<owl:Class>
						<owl:intersectionOf rdf:parseType="Collection">
							<rdf:Description rdf:about="&fibo-der-der-opt;OptionIssuer">
							</rdf:Description>
							<rdf:Description rdf:about="&fibo-der-der-opt;OptionsExchangeParticipant">
							</rdf:Description>
						</owl:intersectionOf>
					</owl:Class>
				</owl:someValuesFrom>
			</owl:Restriction>
		</rdfs:subClassOf>
		<rdfs:subClassOf>
			<owl:Restriction>
				<owl:onProperty rdf:resource="&fibo-sec-dbt-ex;hasExerciseTerms"/>
				<owl:someValuesFrom rdf:resource="&fibo-sec-dbt-ex;ExerciseTerms"/>
			</owl:Restriction>
		</rdfs:subClassOf>
		<rdfs:label xml:lang="en">exchange-traded option</rdfs:label>
		<skos:definition xml:lang="en">standardized option giving the buyer (holder) the right, but not the obligation, to buy (via a call option) or sell (via a put option) the underlying assets specified at a pre-determined price (i.e., the strike price, fixed or calculated), on or before a specified date (the expiration date)</skos:definition>
	</owl:Class>
	
	<owl:Class rdf:about="&fibo-der-der-opt;FixedLookbackStrikeFormula">
		<rdfs:subClassOf rdf:resource="&fibo-der-der-opt;StrikeFormula"/>
		<rdfs:subClassOf>
			<owl:Restriction>
				<owl:onProperty rdf:resource="&fibo-fnd-utl-alx;hasExpression"/>
				<owl:someValuesFrom rdf:resource="&fibo-der-der-opt;FixedLookbackStrikeFormulaExpression"/>
			</owl:Restriction>
		</rdfs:subClassOf>
		<rdfs:label xml:lang="en">fixed lookback strike formula</rdfs:label>
	</owl:Class>
	
	<owl:Class rdf:about="&fibo-der-der-opt;FixedLookbackStrikeFormulaExpression">
		<rdfs:subClassOf rdf:resource="&fibo-der-der-opt;LookbackExpression"/>
		<rdfs:subClassOf>
			<owl:Restriction>
				<owl:onProperty rdf:resource="&fibo-fnd-utl-alx;hasMinuend"/>
				<owl:someValuesFrom rdf:resource="&fibo-der-der-opt;FixedStrikeAmount"/>
			</owl:Restriction>
		</rdfs:subClassOf>
		<rdfs:subClassOf>
			<owl:Restriction>
				<owl:onProperty rdf:resource="&fibo-fnd-utl-alx;hasSubtrahend"/>
				<owl:someValuesFrom rdf:resource="&fibo-der-der-opt;ObservableBestValue"/>
			</owl:Restriction>
		</rdfs:subClassOf>
		<rdfs:label xml:lang="en">fixed lookback strike formula expression</rdfs:label>
	</owl:Class>
	
	<owl:Class rdf:about="&fibo-der-der-opt;FixedLookbackStrikeTerms">
		<rdfs:subClassOf rdf:resource="&fibo-der-der-opt;LookbackStrikeTerms"/>
		<rdfs:subClassOf>
			<owl:Restriction>
				<owl:onProperty rdf:resource="&fibo-fnd-utl-alx;hasFormula"/>
				<owl:someValuesFrom rdf:resource="&fibo-der-der-opt;FixedLookbackStrikeFormula"/>
			</owl:Restriction>
		</rdfs:subClassOf>
		<rdfs:label xml:lang="en">fixed lookback strike terms</rdfs:label>
		<owl:disjointWith rdf:resource="&fibo-der-der-opt;FloatingLookbackStrikeTerms"/>
		<skos:definition xml:lang="en">Strike terms which reflect the difference between a running maximum value of the observable during the lookback period, and the pre-agreed strike. The agreed settlement is based on the difference between these. Further Notes This is only settled in cash and the strike is predetermined at payoff and the payoff is the max diff between the optimal price and the strike price.</skos:definition>
	</owl:Class>
	
	<owl:Class rdf:about="&fibo-der-der-opt;FixedStrikeAmount">
		<rdfs:subClassOf rdf:resource="&fibo-der-drc-bsc;ObservableValue"/>
		<rdfs:label xml:lang="en">fixed strike amount</rdfs:label>
	</owl:Class>
	
	<owl:Class rdf:about="&fibo-der-der-opt;FixedStrikeTerms">
		<rdfs:subClassOf rdf:resource="&fibo-der-der-opt;OptionStrikeTerms"/>
		<rdfs:subClassOf>
			<owl:Restriction>
				<owl:onProperty rdf:resource="&fibo-der-der-opt;includesSpecificationTerm"/>
				<owl:someValuesFrom rdf:resource="&fibo-der-der-opt;StrikePrice"/>
			</owl:Restriction>
		</rdfs:subClassOf>
		<rdfs:label xml:lang="en">fixed strike terms</rdfs:label>
		<owl:disjointWith rdf:resource="&fibo-der-der-opt;ResetableStrikeTerms"/>
		<skos:definition xml:lang="en">Contractual terms setting out a fixed, pre-agreed price or level at which the option is to be struck.</skos:definition>
		<fibo-fnd-utl-av:explanatoryNote xml:lang="en">This is similar to the FpML term for Strike, but there are two other types of Strike specification - look back and reset. FpML strike: &apos;Defines whether it is a price or level at which the option has been, or will be, struck.&apos;</fibo-fnd-utl-av:explanatoryNote>
	</owl:Class>
	
	<owl:Class rdf:about="&fibo-der-der-opt;FloatingLookbackFormulaExpression">
		<rdfs:subClassOf rdf:resource="&fibo-der-der-opt;LookbackExpression"/>
		<rdfs:subClassOf>
			<owl:Restriction>
				<owl:onProperty rdf:resource="&fibo-fnd-utl-alx;hasMinuend"/>
				<owl:someValuesFrom rdf:resource="&fibo-der-der-opt;ObservableFinalValue"/>
			</owl:Restriction>
		</rdfs:subClassOf>
		<rdfs:subClassOf>
			<owl:Restriction>
				<owl:onProperty rdf:resource="&fibo-fnd-utl-alx;hasSubtrahend"/>
				<owl:someValuesFrom rdf:resource="&fibo-der-der-opt;ObservableBestValue"/>
			</owl:Restriction>
		</rdfs:subClassOf>
		<rdfs:label xml:lang="en">floating lookback formula expression</rdfs:label>
	</owl:Class>
	
	<owl:Class rdf:about="&fibo-der-der-opt;FloatingLookbackStrikeFormula">
		<rdfs:subClassOf rdf:resource="&fibo-der-der-opt;StrikeFormula"/>
		<rdfs:subClassOf>
			<owl:Restriction>
				<owl:onProperty rdf:resource="&fibo-fnd-utl-alx;hasExpression"/>
				<owl:someValuesFrom rdf:resource="&fibo-der-der-opt;FloatingLookbackFormulaExpression"/>
			</owl:Restriction>
		</rdfs:subClassOf>
		<rdfs:label xml:lang="en">floating lookback strike formula</rdfs:label>
	</owl:Class>
	
	<owl:Class rdf:about="&fibo-der-der-opt;FloatingLookbackStrikeSchedule">
		<rdfs:subClassOf rdf:resource="&fibo-fnd-dt-fd;Schedule"/>
		<rdfs:label xml:lang="en">floating lookback strike schedule</rdfs:label>
	</owl:Class>
	
	<owl:Class rdf:about="&fibo-der-der-opt;FloatingLookbackStrikeTerms">
		<rdfs:subClassOf rdf:resource="&fibo-der-der-opt;LookbackStrikeTerms"/>
		<rdfs:subClassOf>
			<owl:Restriction>
				<owl:onProperty rdf:resource="&fibo-fnd-utl-alx;hasFormula"/>
				<owl:someValuesFrom rdf:resource="&fibo-der-der-opt;FloatingLookbackStrikeFormula"/>
			</owl:Restriction>
		</rdfs:subClassOf>
		<rdfs:label xml:lang="en">floating lookback strike terms</rdfs:label>
	</owl:Class>
	
	<owl:Class rdf:about="&fibo-der-der-opt;ForeignCurrencyOption">
		<rdfs:subClassOf rdf:resource="&fibo-der-der-opt;ExchangeTradedOption"/>
		<rdfs:subClassOf rdf:resource="&fibo-der-fx-ctr;ForeignExchangeDerivative"/>
		<rdfs:subClassOf>
			<owl:Restriction>
				<owl:onProperty rdf:resource="&fibo-der-drc-bsc;hasUnderlier"/>
				<owl:someValuesFrom rdf:resource="&fibo-der-der-opt;FxOptionUnderlying"/>
			</owl:Restriction>
		</rdfs:subClassOf>
		<rdfs:subClassOf>
			<owl:Restriction>
				<owl:onProperty rdf:resource="&fibo-sec-dbt-ex;hasExerciseTerms"/>
				<owl:someValuesFrom rdf:resource="&fibo-der-der-opt;CurrencyOptionExerciseTerms"/>
			</owl:Restriction>
		</rdfs:subClassOf>
		<rdfs:label xml:lang="en">foreign currency option</rdfs:label>
		<skos:definition xml:lang="en">An option on a currency, based on the spot exchange rate of that currency to the currency of the security itself.</skos:definition>
		<skos:editorialNote xml:lang="en">Definition needed - this is just a place holder. Actually, this would also have a Currency Future as the Underlying Action: change this. Definition:Review</skos:editorialNote>
	</owl:Class>
	
	<owl:Class rdf:about="&fibo-der-der-opt;FutureOptionsExerciseTerms">
		<rdfs:subClassOf rdf:resource="&fibo-sec-dbt-ex;AmericanExerciseTerms"/>
		<rdfs:subClassOf>
			<owl:Restriction>
				<owl:onProperty rdf:resource="&fibo-der-der-opt;delivery"/>
				<owl:someValuesFrom rdf:resource="&fibo-fbc-fi-fi;Future"/>
			</owl:Restriction>
		</rdfs:subClassOf>
		<rdfs:label xml:lang="en">future options exercise terms</rdfs:label>
		<skos:definition xml:lang="en">Contractual terms defining when or under what circumstances an options instrument may be exercised.</skos:definition>
		<fibo-fnd-utl-av:explanatoryNote xml:lang="en">Also includes terms defining delivery when the contract is exercised.</fibo-fnd-utl-av:explanatoryNote>
	</owl:Class>
	
	<owl:Class rdf:about="&fibo-der-der-opt;FxOptionUnderlying">
		<rdfs:subClassOf rdf:resource="&fibo-der-drc-bsc;Underlier"/>
		<rdfs:subClassOf>
			<owl:Restriction>
				<owl:onProperty rdf:resource="&fibo-fnd-rel-rel;hasIdentity"/>
				<owl:someValuesFrom rdf:resource="&fibo-ind-fx-fx;CurrencySpotBuyRate"/>
			</owl:Restriction>
		</rdfs:subClassOf>
		<rdfs:label xml:lang="en">fx option underlying</rdfs:label>
		<skos:definition xml:lang="en">The underlying of the foreign currency option is a currency spot rate.</skos:definition>
	</owl:Class>
	
	<owl:Class rdf:about="&fibo-der-der-opt;IndexOptionExerciseTerms">
		<rdfs:subClassOf rdf:resource="&fibo-sec-dbt-ex;ExerciseTerms"/>
		<rdfs:subClassOf>
			<owl:Restriction>
				<owl:onProperty rdf:resource="&fibo-der-der-opt;delivery"/>
				<owl:someValuesFrom rdf:resource="&fibo-fnd-acc-cur;AmountOfMoney"/>
			</owl:Restriction>
		</rdfs:subClassOf>
		<rdfs:label xml:lang="en">index option exercise terms</rdfs:label>
		<skos:definition xml:lang="en">Contractual terms defining when or under what circumstances an options instrument may be exercised.</skos:definition>
		<fibo-fnd-utl-av:explanatoryNote xml:lang="en">Also includes terms defining delivery when the contract is exercised. Delivery for index options is by way of cash.</fibo-fnd-utl-av:explanatoryNote>
	</owl:Class>
	
	<owl:Class rdf:about="&fibo-der-der-opt;InterestRateOption">
		<rdfs:subClassOf rdf:resource="&fibo-der-der-opt;OptionOnFuture"/>
		<rdfs:subClassOf>
			<owl:Restriction>
				<owl:onProperty rdf:resource="&fibo-der-drc-bsc;hasUnderlier"/>
				<owl:someValuesFrom rdf:resource="&fibo-fnd-acc-cur;InterestRate"/>
			</owl:Restriction>
		</rdfs:subClassOf>
		<rdfs:label xml:lang="en">interest rate option</rdfs:label>
		<skos:definition xml:lang="en">option on some underlying interest rate</skos:definition>
		<fibo-fnd-utl-av:explanatoryNote xml:lang="en">If the option is exercised, delivery is in the form of the corresponding interest rate future.</fibo-fnd-utl-av:explanatoryNote>
	</owl:Class>
	
	<owl:Class rdf:about="&fibo-der-der-opt;KnockIn">
		<rdfs:subClassOf rdf:resource="&fibo-der-der-opt;OptionFeature"/>
		<rdfs:label xml:lang="en">knock in</rdfs:label>
		<skos:definition xml:lang="en">An option which comes into existence if the knock-in event happens. It works exactly the reverse of a knock-out. In a knock-in, an option comes into existence if a certain level is hit.</skos:definition>
	</owl:Class>
	
	<owl:Class rdf:about="&fibo-der-der-opt;KnockOut">
		<rdfs:subClassOf rdf:resource="&fibo-der-der-opt;OptionFeature"/>
		<rdfs:label xml:lang="en">knock out</rdfs:label>
		<skos:definition xml:lang="en">An option which ceases to exist if the knock-out event occurs. A knock out happens when a particular level is hit (like the Swiss franc touching the level of 1.10 against the dollar), when the option ceases to exist.</skos:definition>
	</owl:Class>
	
	<owl:Class rdf:about="&fibo-der-der-opt;LinearPayoutCommitment">
		<rdfs:subClassOf rdf:resource="&fibo-der-der-opt;OptionPayoutCommitment"/>
		<rdfs:label xml:lang="en">linear payout commitment</rdfs:label>
		<skos:definition xml:lang="en">The commitment to pay out on a straight vanilla option.</skos:definition>
	</owl:Class>
	
	<owl:Class rdf:about="&fibo-der-der-opt;LinearPayoutTerms">
		<rdfs:subClassOf rdf:resource="&fibo-der-der-opt;OptionPayoutTerms"/>
		<rdfs:subClassOf>
			<owl:Restriction>
				<owl:onProperty rdf:resource="&fibo-fnd-agr-ctr;definesTermsFor"/>
				<owl:someValuesFrom rdf:resource="&fibo-der-der-opt;LinearPayoutCommitment"/>
			</owl:Restriction>
		</rdfs:subClassOf>
		<rdfs:label xml:lang="en">linear payout terms</rdfs:label>
		<skos:definition xml:lang="en">Terms governing the payment commitment on a vanilla option.</skos:definition>
	</owl:Class>
	
	<owl:Class rdf:about="&fibo-der-der-opt;LongTermEquityOption">
		<rdfs:subClassOf rdf:resource="&fibo-der-der-opt;EquityOption"/>
		<rdfs:subClassOf>
			<owl:Restriction>
				<owl:onProperty rdf:resource="&fibo-fnd-agr-ctr;hasContractDuration"/>
				<owl:someValuesFrom rdf:resource="&fibo-fnd-dt-fd;Duration"/>
			</owl:Restriction>
		</rdfs:subClassOf>
		<rdfs:label xml:lang="en">long term equity option</rdfs:label>
		<skos:definition xml:lang="en">An option whose contract expires at a date longer than one year. Also known as long-term equity anticipation securities (LEAPS). From Investopedia: These options are called long-term equity anticipation securities (LEAPS). By providing opportunities to control and manage risk or even to speculate, LEAPS are virtually identical to regular options. LEAPS, however, provide these opportunities for much longer periods of time. Although they are not available on all stocks, LEAPS are available on most widely held issues.</skos:definition>
	</owl:Class>
	
	<owl:Class rdf:about="&fibo-der-der-opt;LookbackExpression">
		<rdfs:subClassOf rdf:resource="&fibo-fnd-utl-alx;Expression"/>
		<rdfs:label xml:lang="en">lookback expression</rdfs:label>
		<skos:definition xml:lang="en">An expression of a lookback formula</skos:definition>
	</owl:Class>
	
	<owl:Class rdf:about="&fibo-der-der-opt;LookbackObservableValue">
		<rdfs:subClassOf rdf:resource="&fibo-fnd-qt-qtu;QuantityValue"/>
		<rdfs:subClassOf>
			<owl:Restriction>
				<owl:onProperty rdf:resource="&fibo-fnd-dt-fd;hasObservedDateTime"/>
				<owl:someValuesFrom rdf:resource="&fibo-fnd-dt-fd;CombinedDateTime"/>
			</owl:Restriction>
		</rdfs:subClassOf>
		<rdfs:label xml:lang="en">lookback observable value</rdfs:label>
	</owl:Class>
	
	<owl:Class rdf:about="&fibo-der-der-opt;LookbackObservableValueAtMaturity">
		<rdfs:subClassOf rdf:resource="&fibo-der-der-opt;LookbackObservableValue"/>
		<rdfs:label xml:lang="en">lookback observable value at maturity</rdfs:label>
	</owl:Class>
	
	<owl:Class rdf:about="&fibo-der-der-opt;LookbackObservableValueDuringLookbackPeriod">
		<rdfs:subClassOf rdf:resource="&fibo-der-der-opt;LookbackObservableValue"/>
		<rdfs:label xml:lang="en">lookback observable value during lookback period</rdfs:label>
	</owl:Class>
	
	<owl:Class rdf:about="&fibo-der-der-opt;LookbackStrikeObservable">
		<rdfs:subClassOf rdf:resource="&fibo-der-drc-bsc;Underlier"/>
		<rdfs:subClassOf>
			<owl:Restriction>
				<owl:onProperty rdf:resource="&fibo-fnd-rel-rel;hasIdentity"/>
				<owl:someValuesFrom rdf:resource="&fibo-fnd-qt-qtu;QuantityValue"/>
			</owl:Restriction>
		</rdfs:subClassOf>
		<rdfs:label xml:lang="en">lookback strike observable</rdfs:label>
		<skos:definition xml:lang="en">The agreed parameter which is used in the formula for fixed OR floating lookback.</skos:definition>
	</owl:Class>
	
	<owl:Class rdf:about="&fibo-der-der-opt;LookbackStrikeTerms">
		<rdfs:subClassOf rdf:resource="&fibo-der-der-opt;OptionStrikeTerms"/>
		<rdfs:subClassOf>
			<owl:Restriction>
				<owl:onProperty rdf:resource="&fibo-der-der-opt;hasSchedule"/>
				<owl:someValuesFrom rdf:resource="&fibo-der-der-opt;FloatingLookbackStrikeSchedule"/>
			</owl:Restriction>
		</rdfs:subClassOf>
		<rdfs:label xml:lang="en">lookback strike terms</rdfs:label>
		<skos:definition xml:lang="en">Strike terms in which the value of some observed variable (the underlying) is looked back at during some period, typically a period ending in the maturity of the Option, and the payoff is determined by comparing the agreed strike with the value of this variable.</skos:definition>
		<fibo-fnd-utl-av:explanatoryNote xml:lang="en">The payoff may either be the difference between a fixed, pre-agreed Strike Price and the observable, or the difference between the best or worst valuable of the observable and the value of that same observable at maturity of the contract (these are the Fixed and Floating lookback terms respectively). This (per review at Nordea) is not mutually exclusive with the terms for Fixed Strike and Resettable Strike, that is, either of those kinds of strike terms may apply, and Lookback strike terms may also apply.</fibo-fnd-utl-av:explanatoryNote>
	</owl:Class>
	
	<owl:Class rdf:about="&fibo-der-der-opt;NovatedOptionContract">
		<rdfs:subClassOf rdf:resource="&fibo-der-der-opt;ExchangeTradedOption"/>
		<rdfs:subClassOf>
			<owl:Restriction>
				<owl:onProperty rdf:resource="&fibo-fnd-pas-pas;hasSeller"/>
				<owl:someValuesFrom rdf:resource="&fibo-der-der-opt;NovatedOptionContractPrincipal"/>
			</owl:Restriction>
		</rdfs:subClassOf>
		<rdfs:label xml:lang="en">novated option contract</rdfs:label>
		<skos:definition xml:lang="en">An Option Contract after the stage where a Derivatives Exchange has novated this contract and become the principal to it, for purposes of clearing and settlement. The Clearing House novates both contract. So when you are on the floor (as a Broker), you trade with another Broker. Then you take it to th eRing, and present it to the Ring. So you write a contract and give it to the ringleader, who then books it. So the party you dealt with deals with the exahcnge, and you deal with the exchange. THen there are two contracts for one deal. So the answer here is that there are two novated contracts for one Options deal. Difference: If not open outcry? In OO the deal is done and given to the ringleader, who represents the Cleaing house. When it&apos;s not open outcry, the clearing house gets the deal, books the deal, and margins it. So you don&apos;t know as much about the deal and process. This eliminiates stickiness of a market that has credit. Similar to what occurs in share markets, where clearing takes place, e.g. when someone defaults on delivery. Clearing House simply closes out the contract.</skos:definition>
	</owl:Class>
	
	<owl:Class rdf:about="&fibo-der-der-opt;NovatedOptionContractPrincipal">
		<rdfs:subClassOf rdf:resource="&fibo-der-der-opt;TradedOptionPrincipal"/>
		<rdfs:subClassOf>
			<owl:Restriction>
				<owl:onProperty rdf:resource="&fibo-fnd-rel-rel;hasIdentity"/>
				<owl:someValuesFrom>
					<owl:Class>
						<owl:unionOf rdf:parseType="Collection">
							<rdf:Description rdf:about="&fibo-der-drc-bsc;DesignatedContractMarket">
							</rdf:Description>
							<rdf:Description rdf:about="&fibo-der-drc-bsc;DerivativesClearingOrganization">
							</rdf:Description>
						</owl:unionOf>
					</owl:Class>
				</owl:someValuesFrom>
			</owl:Restriction>
		</rdfs:subClassOf>
		<rdfs:label xml:lang="en">novated option contract principal</rdfs:label>
	</owl:Class>
	
	<owl:Class rdf:about="&fibo-der-der-opt;ObservableBestValue">
		<rdfs:subClassOf rdf:resource="&fibo-der-drc-bsc;ObservableValue"/>
		<rdfs:subClassOf>
			<owl:Restriction>
				<owl:onProperty rdf:resource="&fibo-der-der-opt;isOf"/>
				<owl:someValuesFrom rdf:resource="&fibo-der-der-opt;LookbackStrikeObservable"/>
			</owl:Restriction>
		</rdfs:subClassOf>
		<rdfs:subClassOf>
			<owl:Restriction>
				<owl:onProperty rdf:resource="&fibo-fnd-rel-rel;hasIdentity"/>
				<owl:someValuesFrom rdf:resource="&fibo-der-der-opt;LookbackObservableValueDuringLookbackPeriod"/>
			</owl:Restriction>
		</rdfs:subClassOf>
		<rdfs:label xml:lang="en">observable best value</rdfs:label>
	</owl:Class>
	
	<owl:Class rdf:about="&fibo-der-der-opt;ObservableFinalValue">
		<rdfs:subClassOf rdf:resource="&fibo-der-drc-bsc;ObservableValue"/>
		<rdfs:subClassOf>
			<owl:Restriction>
				<owl:onProperty rdf:resource="&fibo-fnd-rel-rel;hasIdentity"/>
				<owl:someValuesFrom rdf:resource="&fibo-der-der-opt;LookbackObservableValueAtMaturity"/>
			</owl:Restriction>
		</rdfs:subClassOf>
		<rdfs:label xml:lang="en">observable final value</rdfs:label>
	</owl:Class>
	
	<owl:Class rdf:about="&fibo-der-der-opt;OptionBarrierFeatureEvent">
		<rdfs:subClassOf rdf:resource="&fibo-fnd-dt-oc;OccurrenceKind"/>
		<rdfs:subClassOf>
			<owl:Restriction>
				<owl:onProperty rdf:resource="&fibo-der-der-opt;hasDirection"/>
				<owl:someValuesFrom rdf:resource="&fibo-der-der-opt;UpOrDown"/>
			</owl:Restriction>
		</rdfs:subClassOf>
		<rdfs:subClassOf>
			<owl:Restriction>
				<owl:onProperty rdf:resource="&fibo-fnd-rel-rel;refersTo"/>
				<owl:someValuesFrom rdf:resource="&fibo-ind-ind-ind;MarketRate"/>
			</owl:Restriction>
		</rdfs:subClassOf>
		<rdfs:label xml:lang="en">option barrier feature event</rdfs:label>
		<skos:definition xml:lang="en">An event which defines when an option feature comes into effect.</skos:definition>
	</owl:Class>
	
	<owl:Class rdf:about="&fibo-der-der-opt;OptionBarrierFeatureTerms">
		<rdfs:subClassOf rdf:resource="&fibo-der-der-opt;OptionTerms"/>
		<rdfs:subClassOf>
			<owl:Restriction>
				<owl:onProperty rdf:resource="&fibo-fbc-fct-ra;specifies"/>
				<owl:someValuesFrom rdf:resource="&fibo-der-der-opt;OptionBarrierFeatureEvent"/>
			</owl:Restriction>
		</rdfs:subClassOf>
		<rdfs:subClassOf>
			<owl:Restriction>
				<owl:onProperty rdf:resource="&fibo-fbc-fct-ra;specifies"/>
				<owl:someValuesFrom rdf:resource="&fibo-der-der-opt;OptionFeature"/>
			</owl:Restriction>
		</rdfs:subClassOf>
		<rdfs:label xml:lang="en">option barrier feature terms</rdfs:label>
		<skos:definition xml:lang="en">Formal terms setting out when and under what circumstances the option contract is deemed to be in force. This takes the form of an event and the relationship between the event and the applicability of the option.</skos:definition>
		<skos:editorialNote xml:lang="en">After some research it was determined that the nature of the thing normally called &quot;Feature&quot; in an option is a contractual term defining when and under what circumstances the option itself is deemed be in force. Option features in this sense are &quot;Knock In&quot; or &quot;Knock Out&quot;, each relating to a market event (usually a price reaching a given level). A third feature, &quot;Knock In Knock Out&quot; is really two of these and is represented as such in the Option terms i.e. there may be two of this Option Feature Terms term. The term &quot;Barrier Option&quot; applies to both of these, i.e. Knock In and Knock Out are types of Barrier Option. An option contract may or may not have a barrier option. If it does not, none of this applies. Others: knock in a knock out, knock in a digitale, if it exceeds one barrier you get a call; for another you get a put, and so on.</skos:editorialNote>
		<fibo-fnd-utl-av:explanatoryNote xml:lang="en">Barrier features include any terms related to exercising the option ahead of the expiry date.</fibo-fnd-utl-av:explanatoryNote>
	</owl:Class>
	
	<owl:Class rdf:about="&fibo-der-der-opt;OptionBinaryPayoutTerms">
		<rdfs:subClassOf rdf:resource="&fibo-der-der-opt;OptionPayoutTerms"/>
		<rdfs:subClassOf>
			<owl:Restriction>
				<owl:onProperty rdf:resource="&fibo-fnd-agr-ctr;definesTermsFor"/>
				<owl:someValuesFrom rdf:resource="&fibo-der-der-opt;BinaryPayoutCommitment"/>
			</owl:Restriction>
		</rdfs:subClassOf>
		<rdfs:label xml:lang="en">option binary payout terms</rdfs:label>
		<skos:definition xml:lang="en">Terms governing a binary payout commitment.</skos:definition>
	</owl:Class>
	
	<owl:Class rdf:about="&fibo-der-der-opt;OptionConditionalPayoutTerms">
		<rdfs:subClassOf rdf:resource="&fibo-der-der-opt;OptionPayoutTerms"/>
		<rdfs:subClassOf>
			<owl:Restriction>
				<owl:onProperty rdf:resource="&fibo-fnd-agr-ctr;definesTermsFor"/>
				<owl:someValuesFrom rdf:resource="&fibo-der-der-opt;ConditionalPayoutCommitment"/>
			</owl:Restriction>
		</rdfs:subClassOf>
		<rdfs:label xml:lang="en">option conditional payout terms</rdfs:label>
		<skos:definition xml:lang="en">Terms governing a conditional payment commitment on an option.</skos:definition>
	</owl:Class>
	
	<owl:Class rdf:about="&fibo-der-der-opt;OptionFeature">
		<rdfs:subClassOf rdf:resource="&fibo-fnd-gao-obj;Strategy"/>
		<rdfs:label xml:lang="en">option feature</rdfs:label>
		<skos:definition xml:lang="en">Types of feature for an option. This itemizes whether the option comes into force (Knock In) or ceases being in force (Knock Out) when the stated event occurs.</skos:definition>
	</owl:Class>
	
	<owl:Class rdf:about="&fibo-der-der-opt;OptionGuarantor">
		<rdfs:subClassOf rdf:resource="&fibo-fbc-dae-gty;Guarantor"/>
		<rdfs:subClassOf>
			<owl:Restriction>
				<owl:onProperty rdf:resource="&fibo-fnd-rel-rel;hasIdentity"/>
				<owl:someValuesFrom>
					<owl:Class>
						<owl:unionOf rdf:parseType="Collection">
							<rdf:Description rdf:about="&fibo-der-drc-bsc;DesignatedContractMarket">
							</rdf:Description>
							<rdf:Description rdf:about="&fibo-der-drc-bsc;DerivativesClearingOrganization">
							</rdf:Description>
						</owl:unionOf>
					</owl:Class>
				</owl:someValuesFrom>
			</owl:Restriction>
		</rdfs:subClassOf>
		<rdfs:label xml:lang="en">option guarantor</rdfs:label>
		<skos:definition xml:lang="en">guarntor that is an options exchange or clearinghouse that guarantees fulfillment of the terms of the option</skos:definition>
		<fibo-fnd-utl-av:explanatoryNote xml:lang="en">In other words, the exchange or clearinghouse guarantees the trade with respect to any losses incurred by the holder in the event of a default by the issuer, not the value of the underlying asset.</fibo-fnd-utl-av:explanatoryNote>
	</owl:Class>
	
	<owl:Class rdf:about="&fibo-der-der-opt;OptionHolder">
		<rdfs:subClassOf rdf:resource="&fibo-fnd-oac-own;Owner"/>
		<rdfs:subClassOf>
			<owl:Restriction>
				<owl:onProperty rdf:resource="&fibo-fnd-rel-rel;holds"/>
				<owl:someValuesFrom rdf:resource="&fibo-fbc-fi-fi;Option"/>
			</owl:Restriction>
		</rdfs:subClassOf>
		<rdfs:label xml:lang="en">option holder</rdfs:label>
		<skos:definition xml:lang="en">party that owns an option</skos:definition>
		<fibo-fnd-utl-av:explanatoryNote xml:lang="en">In a call, the option holder has the right, but not the obligation, to buy the underlying asset, while, in a put, the option holder has the right to sell the underlying asset. An option holder may sell the option contract itself, at which point the buyer becomes the option holder. The holder has an obligation to inform the seller by a certain time if they wish to exercise. Once the instrument is exercised there are typically additional, relevant obligations with regard to settlement.</fibo-fnd-utl-av:explanatoryNote>
	</owl:Class>
	
	<owl:Class rdf:about="&fibo-der-der-opt;OptionIssuer">
		<rdfs:subClassOf rdf:resource="&fibo-fbc-fi-fi;Issuer"/>
		<rdfs:subClassOf>
			<owl:Restriction>
				<owl:onProperty rdf:resource="&fibo-fnd-pty-rl;isPlayedBy"/>
				<owl:someValuesFrom>
					<owl:Restriction>
						<owl:onProperty rdf:resource="&fibo-fnd-pty-pty;isAPartyTo"/>
						<owl:someValuesFrom rdf:resource="&fibo-fbc-fi-fi;Option"/>
					</owl:Restriction>
				</owl:someValuesFrom>
			</owl:Restriction>
		</rdfs:subClassOf>
		<rdfs:label xml:lang="en">option issuer</rdfs:label>
		<skos:definition xml:lang="en">issuer granting the rights defined in the option in exchange for some consideration</skos:definition>
	</owl:Class>
	
	<owl:Class rdf:about="&fibo-der-der-opt;OptionOnFuture">
		<rdfs:subClassOf rdf:resource="&fibo-fbc-fi-fi;Option"/>
		<rdfs:subClassOf>
			<owl:Restriction>
				<owl:onProperty rdf:resource="&fibo-der-drc-bsc;hasUnderlier"/>
				<owl:someValuesFrom rdf:resource="&fibo-fbc-fi-fi;Future"/>
			</owl:Restriction>
		</rdfs:subClassOf>
		<rdfs:subClassOf>
			<owl:Restriction>
				<owl:onProperty rdf:resource="&fibo-sec-dbt-ex;hasExerciseTerms"/>
				<owl:someValuesFrom rdf:resource="&fibo-der-der-opt;FutureOptionsExerciseTerms"/>
			</owl:Restriction>
		</rdfs:subClassOf>
		<rdfs:label xml:lang="en">option on future</rdfs:label>
		<skos:definition xml:lang="en">option that gives the holder the right, but not the obligation, to buy or sell a specific futures contract at a specified price on or before the option&apos;s expiration date</skos:definition>
	</owl:Class>
	
	<owl:Class rdf:about="&fibo-der-der-opt;OptionPayoutCommitment">
		<rdfs:subClassOf rdf:resource="&fibo-fnd-agr-ctr;ContractualCommitment"/>
		<rdfs:subClassOf>
			<owl:Restriction>
				<owl:onProperty rdf:resource="&fibo-der-der-opt;enteredIntoBy"/>
				<owl:someValuesFrom rdf:resource="&fibo-der-der-opt;OptionIssuer"/>
			</owl:Restriction>
		</rdfs:subClassOf>
		<rdfs:label xml:lang="en">option payout commitment</rdfs:label>
		<skos:definition xml:lang="en">Commitment by the issuer to pay out on an option should the holder choose to exercise this.</skos:definition>
		<fibo-fnd-utl-av:explanatoryNote xml:lang="en">This commitment is set out in formal Exercise Terms.</fibo-fnd-utl-av:explanatoryNote>
	</owl:Class>
	
	<owl:Class rdf:about="&fibo-der-der-opt;OptionPayoutTerms">
		<rdfs:subClassOf rdf:resource="&fibo-der-drc-bsc;ParametricCashflowTerms"/>
		<rdfs:subClassOf rdf:resource="&fibo-der-der-opt;OptionTerms"/>
		<rdfs:subClassOf>
			<owl:Restriction>
				<owl:onProperty rdf:resource="&fibo-fnd-agr-ctr;definesTermsFor"/>
				<owl:someValuesFrom rdf:resource="&fibo-der-der-opt;OptionPayoutCommitment"/>
			</owl:Restriction>
		</rdfs:subClassOf>
		<rdfs:label xml:lang="en">option payout terms</rdfs:label>
		<skos:definition xml:lang="en">Terms governing the payout on an option. These formally define the commitment(s) entered into by the writing party to the option.</skos:definition>
	</owl:Class>
	
	<owl:Class rdf:about="&fibo-der-der-opt;OptionPremium">
		<rdfs:subClassOf rdf:resource="&fibo-fbc-fi-ip;MarketPrice"/>
		<rdfs:subClassOf rdf:resource="&fibo-fnd-acc-cur;CalculatedPrice"/>
		<rdfs:subClassOf>
			<owl:Restriction>
				<owl:onProperty rdf:resource="&fibo-fnd-utl-alx;hasFormula"/>
				<owl:onClass rdf:resource="&fibo-der-der-opt;OptionPremiumFormula"/>
				<owl:minQualifiedCardinality rdf:datatype="&xsd;nonNegativeInteger">0</owl:minQualifiedCardinality>
			</owl:Restriction>
		</rdfs:subClassOf>
		<rdfs:subClassOf>
			<owl:Restriction>
				<owl:onProperty rdf:resource="&fibo-fnd-acc-cur;hasMonetaryAmount"/>
				<owl:onClass rdf:resource="&fibo-fnd-acc-cur;MonetaryAmount"/>
				<owl:minQualifiedCardinality rdf:datatype="&xsd;nonNegativeInteger">0</owl:minQualifiedCardinality>
			</owl:Restriction>
		</rdfs:subClassOf>
		<rdfs:subClassOf>
			<owl:Restriction>
				<owl:onProperty rdf:resource="&fibo-fnd-qt-qtu;hasQuantityValue"/>
				<owl:onClass rdf:resource="&fibo-fnd-acc-cur;PercentageMonetaryAmount"/>
				<owl:minQualifiedCardinality rdf:datatype="&xsd;nonNegativeInteger">0</owl:minQualifiedCardinality>
			</owl:Restriction>
		</rdfs:subClassOf>
		<rdfs:subClassOf>
			<owl:Restriction>
				<owl:onProperty rdf:resource="&fibo-der-der-opt;hasRelativePaymentDate"/>
				<owl:someValuesFrom rdf:resource="&fibo-fnd-dt-fd;RelativeDate"/>
			</owl:Restriction>
		</rdfs:subClassOf>
		<rdfs:label xml:lang="en">option premium</rdfs:label>
		<skos:definition xml:lang="en">current market price of an option contract</skos:definition>
		<fibo-fnd-utl-av:explanatoryNote xml:lang="en">The option premium is the income received by the seller (writer) of an option contract to another party. In-the-money option premiums are composed of two factors: intrinsic and extrinsic value. Out-of-the-money options&apos; premiums consist solely of extrinsic value. For stock options, the premium is quoted as a dollar amount per share, and most contracts represent the commitment of 100 shares.</fibo-fnd-utl-av:explanatoryNote>
	</owl:Class>
	
	<owl:Class rdf:about="&fibo-der-der-opt;OptionPremiumFormula">
		<rdfs:subClassOf rdf:resource="&fibo-fnd-utl-alx;Formula"/>
		<rdfs:label xml:lang="en">option premium formula</rdfs:label>
		<skos:definition xml:lang="en">formula used to calculate the premium</skos:definition>
		<fibo-fnd-utl-av:explanatoryNote xml:lang="en">This is a choice between expressing amount of premium paid as either price per option, or percentage of notional amount. FpML: &apos;Choice between expressing amount of premium paid as either price per option, or percentage of notional amount.&apos;</fibo-fnd-utl-av:explanatoryNote>
	</owl:Class>
	
	<owl:Class rdf:about="&fibo-der-der-opt;OptionPremiumPaymentArrangement">
		<rdfs:subClassOf rdf:resource="&fibo-fnd-gao-obj;Strategy"/>
		<rdfs:label xml:lang="en">option premium payment arrangement</rdfs:label>
		<skos:definition xml:lang="en">Premium Type for Forward Start Equity Options.</skos:definition>
		<skos:editorialNote xml:lang="en">This was originally a selectable list called option premium type selection (option premium type in data models). Note against that element is given below, based on which this has been implemented as two sets of classes (both characterized as kinds of method). 

Earlier SME Review note:
Further notes: REVIEW THIS - there appear to be two separate semantics in this list; are they mutually exclusive? Answers: You can pay the premium up front or in arrears (pre v pos tpaid) or you can pay it at any agreed time (indeed the time is already defined as terms see Payment Date), so this simply reflects that. Then there are other types of &quot;Participating OptionS&quot; where the anmount you pay depends on something else - so you don&apos;t pay the Premium up front. If it ends up outt of the money then you don&apos;t have to pay as much. So this is &quot;Variable&quot; premium. The alternative to this is &quot;Fixed&quot;. If it&apos;s prepaid it&apos;s firxed If it&apos;s post paid it can bt variable or fixed. SO these are two facts. FpML: Premium Type for Forward Start Equity Option</skos:editorialNote>
	</owl:Class>
	
	<owl:Class rdf:about="&fibo-der-der-opt;OptionPremiumPreOrPostType">
		<rdfs:subClassOf rdf:resource="&fibo-der-der-opt;OptionPremiumPaymentArrangement"/>
		<rdfs:label xml:lang="en">option premium pre or post type</rdfs:label>
	</owl:Class>
	
	<owl:Class rdf:about="&fibo-der-der-opt;OptionStrikeResetSchedule">
		<rdfs:subClassOf rdf:resource="&fibo-fnd-dt-fd;Schedule"/>
		<rdfs:label xml:lang="en">option strike reset schedule</rdfs:label>
	</owl:Class>
	
	<owl:Class rdf:about="&fibo-der-der-opt;OptionStrikeTerms">
		<rdfs:subClassOf rdf:resource="&fibo-der-der-opt;OptionTerms"/>
		<rdfs:label xml:lang="en">option strike terms</rdfs:label>
		<skos:definition xml:lang="en">Contractual terms setting out the price or level at which the option is to be struck. FpML strike: &apos;Defines whether it is a price or level at which the option has been, or will be, struck.&apos;</skos:definition>
	</owl:Class>
	
	<owl:Class rdf:about="&fibo-der-der-opt;OptionTerms">
		<rdfs:subClassOf rdf:resource="&fibo-der-drc-bsc;DerivativeTerms"/>
		<rdfs:subClassOf>
			<owl:Restriction>
				<owl:onProperty rdf:resource="&fibo-fbc-fct-ra;specifies"/>
				<owl:someValuesFrom rdf:resource="&fibo-sec-dbt-ex;ExerciseTerms"/>
			</owl:Restriction>
		</rdfs:subClassOf>
		<rdfs:label xml:lang="en">option terms</rdfs:label>
	</owl:Class>
	
	<owl:Class rdf:about="&fibo-der-der-opt;OptionsExchangeParticipant">
		<rdfs:subClassOf rdf:resource="&fibo-fnd-pty-pty;PartyInRole"/>
		<rdfs:label xml:lang="en">options exchange participant</rdfs:label>
	</owl:Class>
	
	<owl:Class rdf:about="&fibo-der-der-opt;OptionsListing">
		<rdfs:subClassOf rdf:resource="&fibo-sec-sec-lst;Listing"/>
		<rdfs:subClassOf>
			<owl:Restriction>
				<owl:onProperty rdf:resource="&fibo-fnd-rel-rel;isProvidedBy"/>
				<owl:allValuesFrom>
					<owl:Class>
						<owl:unionOf rdf:parseType="Collection">
							<rdf:Description rdf:about="&fibo-der-drc-bsc;DesignatedContractMarket">
							</rdf:Description>
							<rdf:Description rdf:about="&fibo-der-drc-bsc;DerivativesClearingOrganization">
							</rdf:Description>
						</owl:unionOf>
					</owl:Class>
				</owl:allValuesFrom>
			</owl:Restriction>
		</rdfs:subClassOf>
		<rdfs:label xml:lang="en">options listing</rdfs:label>
		<skos:definition xml:lang="en">A listing of an options instrument on a derivatives exchange. The listing is a product of the individual exchange.</skos:definition>
		<skos:editorialNote xml:lang="en">This term sdoes not exist. If there was a listing of something that was an option, it would be a warrant. Review: We agreed to come back to this definition and verify whether it means the same as listing in the equities sense .</skos:editorialNote>
	</owl:Class>
	
	<owl:Class rdf:about="&fibo-der-der-opt;PayoffAssetsList">
		<rdfs:subClassOf rdf:resource="&fibo-der-sbd-sbd;SecurityUnderlier"/>
		<rdfs:label xml:lang="en">payoff assets list</rdfs:label>
		<skos:definition xml:lang="en">The list of n assets which are used to determine a best or worst value in determining conditinal payoff commitments.</skos:definition>
	</owl:Class>
	
	<owl:Class rdf:about="&fibo-der-der-opt;PutOption">
		<rdfs:subClassOf rdf:resource="&fibo-fbc-fi-fi;Option"/>
		<rdfs:subClassOf>
			<owl:Restriction>
				<owl:onProperty rdf:resource="&fibo-fnd-pas-pas;hasBuyer"/>
				<owl:someValuesFrom>
					<owl:Class>
						<owl:unionOf rdf:parseType="Collection">
							<rdf:Description rdf:about="&fibo-der-der-opt;OptionHolder">
							</rdf:Description>
							<rdf:Description rdf:about="&fibo-der-drc-bsc;ReceivingParty">
							</rdf:Description>
						</owl:unionOf>
					</owl:Class>
				</owl:someValuesFrom>
			</owl:Restriction>
		</rdfs:subClassOf>
		<rdfs:subClassOf>
			<owl:Restriction>
				<owl:onProperty rdf:resource="&fibo-fnd-pas-pas;hasSeller"/>
				<owl:someValuesFrom>
					<owl:Class>
						<owl:unionOf rdf:parseType="Collection">
							<rdf:Description rdf:about="&fibo-der-der-opt;OptionIssuer">
							</rdf:Description>
							<rdf:Description rdf:about="&fibo-der-drc-bsc;PayingParty">
							</rdf:Description>
						</owl:unionOf>
					</owl:Class>
				</owl:someValuesFrom>
			</owl:Restriction>
		</rdfs:subClassOf>
		<rdfs:label xml:lang="en">put option</rdfs:label>
		<skos:definition xml:lang="en">option giving the buyer (holder) the right, but not the obligation, to to sell the assets specified at a fixed price or formula, on or before a specified date</skos:definition>
		<fibo-fnd-utl-av:adaptedFrom xml:lang="en">ISO 10962, Securities and related financial instruments - Classification of financial instruments (CFI) code, Fourth Edition, 2019.</fibo-fnd-utl-av:adaptedFrom>
		<fibo-fnd-utl-av:explanatoryNote xml:lang="en">The seller of the put option assumes the obligation of buying the assets specified should the buyer exercise his or her option.</fibo-fnd-utl-av:explanatoryNote>
	</owl:Class>
	
	<owl:Class rdf:about="&fibo-der-der-opt;ResetableStrikeTerms">
		<rdfs:subClassOf rdf:resource="&fibo-der-der-opt;OptionStrikeTerms"/>
		<rdfs:subClassOf>
			<owl:Restriction>
				<owl:onProperty rdf:resource="&fibo-der-der-opt;hasResetSchedule"/>
				<owl:someValuesFrom rdf:resource="&fibo-der-der-opt;OptionStrikeResetSchedule"/>
			</owl:Restriction>
		</rdfs:subClassOf>
		<rdfs:label xml:lang="en">resetable strike terms</rdfs:label>
	</owl:Class>
	
	<owl:Class rdf:about="&fibo-der-der-opt;SingleStockOption">
		<rdfs:subClassOf rdf:resource="&fibo-der-der-opt;EquityOption"/>
		<rdfs:label xml:lang="en">single stock option</rdfs:label>
		<skos:definition xml:lang="en">Option instrument based on a single equity security (share) underlying.</skos:definition>
	</owl:Class>
	
	<owl:Class rdf:about="&fibo-der-der-opt;StandardizedExerciseTerms">
		<rdfs:subClassOf rdf:resource="&fibo-der-der-opt;StandardizedOptionsTerms"/>
		<rdfs:subClassOf rdf:resource="&fibo-sec-dbt-ex;ExerciseTerms"/>
		<rdfs:subClassOf>
			<owl:Restriction>
				<owl:onProperty rdf:resource="&fibo-fbc-fct-ra;specifies"/>
				<owl:someValuesFrom rdf:resource="&fibo-fbc-fi-fi;FinancialInstrument"/>
			</owl:Restriction>
		</rdfs:subClassOf>
		<rdfs:label xml:lang="en">standardized exercise terms</rdfs:label>
		<skos:definition xml:lang="en">Standard exercise terms for an option contract, determined in advance by the exchange. These will become exercise terms of an individual option contract. These may be varied or overridden for individual contracts.</skos:definition>
	</owl:Class>
	
	<owl:Class rdf:about="&fibo-der-der-opt;StandardizedOptionsTerms">
		<rdfs:subClassOf rdf:resource="&fibo-fbc-fi-fi;StandardizedTerms"/>
		<rdfs:subClassOf>
			<owl:Restriction>
				<owl:onProperty rdf:resource="&fibo-fnd-rel-rel;comprises"/>
				<owl:onClass rdf:resource="&fibo-der-der-opt;OptionBarrierFeatureTerms"/>
				<owl:maxQualifiedCardinality rdf:datatype="&xsd;nonNegativeInteger">2</owl:maxQualifiedCardinality>
			</owl:Restriction>
		</rdfs:subClassOf>
		<rdfs:subClassOf>
			<owl:Restriction>
				<owl:onProperty rdf:resource="&fibo-be-fct-pub;hasPublisher"/>
				<owl:someValuesFrom>
					<owl:Class>
						<owl:unionOf rdf:parseType="Collection">
							<rdf:Description rdf:about="&fibo-fbc-fct-mkt;Exchange">
							</rdf:Description>
							<rdf:Description rdf:about="&fibo-der-drc-bsc;DerivativesClearingOrganization">
							</rdf:Description>
						</owl:unionOf>
					</owl:Class>
				</owl:someValuesFrom>
			</owl:Restriction>
		</rdfs:subClassOf>
		<rdfs:subClassOf>
			<owl:Restriction>
				<owl:onProperty rdf:resource="&fibo-fbc-fi-ip;hasPriceDeterminationMethod"/>
				<owl:someValuesFrom rdf:resource="&fibo-fbc-fi-ip;PriceDeterminationMethod"/>
			</owl:Restriction>
		</rdfs:subClassOf>
		<rdfs:subClassOf>
			<owl:Restriction>
				<owl:onProperty rdf:resource="&fibo-fnd-rel-rel;appliesTo"/>
				<owl:someValuesFrom rdf:resource="&fibo-der-der-opt;ExchangeTradedOption"/>
			</owl:Restriction>
		</rdfs:subClassOf>
		<rdfs:label xml:lang="en">standardized options terms</rdfs:label>
		<skos:definition xml:lang="en">standardized contract terms established by a securities or options exchange or by an options clearing entity</skos:definition>
		<fibo-fnd-utl-av:adaptedFrom xml:lang="en">ISO 10962, Securities and related financial instruments - Classification of financial instruments (CFI) code, Fourth Edition, 2019.</fibo-fnd-utl-av:adaptedFrom>
		<fibo-fnd-utl-av:explanatoryNote xml:lang="en">Such terms may relate to the underlying instruments, exercise price, expiration date, and contract size, for example.</fibo-fnd-utl-av:explanatoryNote>
	</owl:Class>
	
	<owl:Class rdf:about="&fibo-der-der-opt;StockOptionExerciseTerms">
		<rdfs:subClassOf rdf:resource="&fibo-sec-dbt-ex;ExerciseTerms"/>
		<rdfs:subClassOf>
			<owl:Restriction>
				<owl:onProperty rdf:resource="&fibo-der-der-opt;delivery"/>
				<owl:someValuesFrom rdf:resource="&fibo-sec-eq-eq;ListedShare"/>
			</owl:Restriction>
		</rdfs:subClassOf>
		<rdfs:label xml:lang="en">stock option exercise terms</rdfs:label>
		<skos:definition xml:lang="en">Contractual terms defining when or under what circumstances a single stock options instrument may be exercised.</skos:definition>
		<fibo-fnd-utl-av:explanatoryNote xml:lang="en">Delivery when the contract is exercised is by delivery of the underlying stock. ADD: Delivery dates, as being distinct from exercise dates.</fibo-fnd-utl-av:explanatoryNote>
	</owl:Class>
	
	<owl:Class rdf:about="&fibo-der-der-opt;StrikeFormula">
		<rdfs:subClassOf rdf:resource="&fibo-der-drc-bsc;CashflowFormula"/>
		<rdfs:label xml:lang="en">strike formula</rdfs:label>
	</owl:Class>
	
	<owl:Class rdf:about="&fibo-der-der-opt;StrikePrice">
		<rdfs:subClassOf rdf:resource="&fibo-fnd-acc-cur;MonetaryPrice"/>
		<rdfs:label xml:lang="en">strike price</rdfs:label>
		<skos:definition xml:lang="en">The strike price for the option is the agreed price for the transaction if this takes place. Applies to all options types. Action: Make sure that&apos;s there for all Options types.</skos:definition>
	</owl:Class>
	
	<owl:Class rdf:about="&fibo-der-der-opt;Swaption">
		<rdfs:subClassOf rdf:resource="&fibo-fbc-fi-fi;Option"/>
		<rdfs:subClassOf>
			<owl:Restriction>
				<owl:onProperty rdf:resource="&fibo-der-drc-bsc;hasUnderlier"/>
				<owl:someValuesFrom rdf:resource="&fibo-der-drc-swp;Swap"/>
			</owl:Restriction>
		</rdfs:subClassOf>
		<rdfs:label xml:lang="en">swaption</rdfs:label>
		<skos:definition xml:lang="en">over-the-counter option that confers the right but not the obligation, to enter into a swap transaction at some time in the future</skos:definition>
		<fibo-fnd-utl-av:explanatoryNote xml:lang="en">A swaption, also known as a swap option, refers to an option to enter into an interest rate swap or some other type of swap. In exchange for an options premium, the buyer gains the right but not the obligation to enter into a specified swap agreement with the issuer on a specified future date.</fibo-fnd-utl-av:explanatoryNote>
		<fibo-fnd-utl-av:synonym xml:lang="en">swap option</fibo-fnd-utl-av:synonym>
	</owl:Class>
	
	<owl:Class rdf:about="&fibo-der-der-opt;TradedOptionPrincipal">
		<rdfs:subClassOf rdf:resource="&fibo-der-der-opt;OptionIssuer"/>
		<rdfs:subClassOf rdf:resource="&fibo-der-der-opt;OptionsExchangeParticipant"/>
		<rdfs:label xml:lang="en">traded option principal</rdfs:label>
		<owl:disjointWith rdf:resource="&fibo-der-der-opt;TradedOptionsCounterparty"/>
		<skos:definition xml:lang="en">The principal to the Traded Option contract. THis is the party which gives the other party the right to take up the obligation, and which is obliged to honor that transaction if that option is taken up.</skos:definition>
	</owl:Class>
	
	<owl:Class rdf:about="&fibo-der-der-opt;TradedOptionsCounterparty">
		<rdfs:subClassOf rdf:resource="&fibo-der-der-opt;OptionHolder"/>
		<rdfs:subClassOf rdf:resource="&fibo-der-der-opt;OptionsExchangeParticipant"/>
		<rdfs:label xml:lang="en">traded options counterparty</rdfs:label>
	</owl:Class>
	
	<owl:Class rdf:about="&fibo-der-der-opt;UnderlyingAssetBuyer">
		<rdfs:subClassOf rdf:resource="&fibo-fnd-pas-pas;Buyer"/>
		<rdfs:label xml:lang="en">underlying asset buyer</rdfs:label>
		<skos:definition xml:lang="en">buyer of the underlying asset in an option-related transaction</skos:definition>
		<fibo-fnd-utl-av:explanatoryNote xml:lang="en">This is the party which buys the underlying in the event that the transaction goes ahead.</fibo-fnd-utl-av:explanatoryNote>
	</owl:Class>
	
	<owl:Class rdf:about="&fibo-der-der-opt;UnderlyingAssetSeller">
		<rdfs:subClassOf rdf:resource="&fibo-fnd-pas-pas;Seller"/>
		<rdfs:label xml:lang="en">underlying asset seller</rdfs:label>
		<skos:definition xml:lang="en">seller of the underlying asset in an option-related transaction</skos:definition>
	</owl:Class>
	
	<owl:Class rdf:about="&fibo-der-der-opt;UpOrDown">
		<rdfs:label xml:lang="en">up or down</rdfs:label>
	</owl:Class>
	
	<owl:ObjectProperty rdf:about="&fibo-der-der-opt;delivery">
		<rdfs:label xml:lang="en">delivery</rdfs:label>
		<rdfs:domain rdf:resource="&fibo-sec-dbt-ex;ExerciseTerms"/>
		<rdfs:range rdf:resource="&fibo-fbc-fi-fi;FinancialInstrument"/>
	</owl:ObjectProperty>
	
	<owl:ObjectProperty rdf:about="&fibo-der-der-opt;enteredIntoBy">
		<rdfs:label xml:lang="en">entered into by</rdfs:label>
		<rdfs:domain rdf:resource="&fibo-der-der-opt;OptionPayoutCommitment"/>
		<rdfs:range rdf:resource="&fibo-der-der-opt;OptionIssuer"/>
	</owl:ObjectProperty>
	
	<owl:DatatypeProperty rdf:about="&fibo-der-der-opt;fixedStrikeAmount">
		<rdfs:label xml:lang="en">fixed strike amount</rdfs:label>
		<rdfs:domain rdf:resource="&fibo-der-der-opt;FixedStrikeAmount"/>
		<rdfs:range rdf:resource="&xsd;decimal"/>
	</owl:DatatypeProperty>
	
	<owl:ObjectProperty rdf:about="&fibo-der-der-opt;hasDirection">
		<rdfs:label xml:lang="en">has direction</rdfs:label>
		<rdfs:domain rdf:resource="&fibo-der-der-opt;OptionBarrierFeatureEvent"/>
		<rdfs:range rdf:resource="&fibo-der-der-opt;UpOrDown"/>
	</owl:ObjectProperty>
	
	<owl:ObjectProperty rdf:about="&fibo-der-der-opt;hasExercisePrice">
		<rdfs:subPropertyOf rdf:resource="&fibo-fnd-acc-cur;hasPrice"/>
		<rdfs:label xml:lang="en">has exercise price</rdfs:label>
		<rdfs:range rdf:resource="&fibo-fnd-acc-cur;MonetaryPrice"/>
		<skos:definition xml:lang="en">predetermined price at which the holder commits to buy or sell an underlying asset</skos:definition>
		<fibo-fnd-utl-av:synonym xml:lang="en">has strike price</fibo-fnd-utl-av:synonym>
	</owl:ObjectProperty>
	
	<owl:ObjectProperty rdf:about="&fibo-der-der-opt;hasOptionTypeElectionDate">
		<rdfs:subPropertyOf rdf:resource="&fibo-fnd-dt-fd;hasExplicitDate"/>
		<rdfs:label xml:lang="en">has option type election date</rdfs:label>
		<rdfs:domain rdf:resource="&fibo-der-der-opt;ChooserOption"/>
		<rdfs:range rdf:resource="&fibo-fnd-dt-fd;ExplicitDate"/>
		<skos:definition xml:lang="en">The date on which the holder of the Chooser option contract determines a choice of either a Call or a Put,</skos:definition>
		<fibo-fnd-utl-av:explanatoryNote xml:lang="en">FpML: &apos;Date where the holder of a Chooser option contract determines a choice of either a Call or a Put&apos;</fibo-fnd-utl-av:explanatoryNote>
	</owl:ObjectProperty>
	
	<owl:ObjectProperty rdf:about="&fibo-der-der-opt;hasPayer">
		<rdfs:label xml:lang="en">has payer</rdfs:label>
		<rdfs:range rdf:resource="&fibo-der-drc-bsc;PayingParty"/>
	</owl:ObjectProperty>
	
	<owl:ObjectProperty rdf:about="&fibo-der-der-opt;hasPremium">
		<rdfs:label xml:lang="en">has premium</rdfs:label>
		<rdfs:domain rdf:resource="&fibo-fbc-fi-fi;Option"/>
		<rdfs:range rdf:resource="&fibo-der-der-opt;OptionPremium"/>
	</owl:ObjectProperty>
	
	<owl:ObjectProperty rdf:about="&fibo-der-der-opt;hasPremiumType">
		<rdfs:label xml:lang="en">has premium type</rdfs:label>
		<rdfs:domain rdf:resource="&fibo-der-der-opt;OptionPremium"/>
		<rdfs:range rdf:resource="&fibo-der-der-opt;OptionPremiumPaymentArrangement"/>
		<skos:definition xml:lang="en">The type of premium payment. FpML: &apos;Premium type for a forward starting equity option.&apos;</skos:definition>
	</owl:ObjectProperty>
	
	<owl:ObjectProperty rdf:about="&fibo-der-der-opt;hasReceiver">
		<rdfs:label xml:lang="en">has receiver</rdfs:label>
		<rdfs:range rdf:resource="&fibo-der-drc-bsc;ReceivingParty"/>
	</owl:ObjectProperty>
	
	<owl:ObjectProperty rdf:about="&fibo-der-der-opt;hasRelativePaymentDate">
		<rdfs:subPropertyOf rdf:resource="&fibo-fnd-dt-fd;hasDate"/>
		<rdfs:label xml:lang="en">has relative payment date</rdfs:label>
		<rdfs:range rdf:resource="&fibo-fnd-dt-fd;RelativeDate"/>
		<skos:definition xml:lang="en">The payment date for the Option Premium.</skos:definition>
		<fibo-fnd-utl-av:explanatoryNote xml:lang="en">This can be expressed as either an adjustable or relative date. FpML: &apos;The payment date, which can be expressed as either an adjustable or relative date.&apos;</fibo-fnd-utl-av:explanatoryNote>
	</owl:ObjectProperty>
	
	<owl:ObjectProperty rdf:about="&fibo-der-der-opt;hasResetSchedule">
		<rdfs:label xml:lang="en">has reset schedule</rdfs:label>
		<rdfs:domain rdf:resource="&fibo-der-der-opt;ResetableStrikeTerms"/>
		<rdfs:range rdf:resource="&fibo-der-der-opt;OptionStrikeResetSchedule"/>
	</owl:ObjectProperty>
	
	<owl:ObjectProperty rdf:about="&fibo-der-der-opt;hasSchedule">
		<rdfs:label xml:lang="en">has schedule</rdfs:label>
		<rdfs:domain rdf:resource="&fibo-der-der-opt;LookbackStrikeTerms"/>
		<rdfs:range rdf:resource="&fibo-der-der-opt;FloatingLookbackStrikeSchedule"/>
	</owl:ObjectProperty>
	
	<owl:ObjectProperty rdf:about="&fibo-der-der-opt;hasStrikePercentageAmount">
		<rdfs:subPropertyOf rdf:resource="&fibo-fnd-acc-cur;hasPrice"/>
		<rdfs:label xml:lang="en">has strike percentage amount</rdfs:label>
		<rdfs:range rdf:resource="&fibo-fnd-acc-cur;PercentageMonetaryAmount"/>
		<skos:definition xml:lang="en">strike price or level expressed as a percentage of the value of the underlying asset</skos:definition>
	</owl:ObjectProperty>
	
	<owl:ObjectProperty rdf:about="&fibo-der-der-opt;hasStrikeTerms">
		<rdfs:subPropertyOf rdf:resource="&fibo-fnd-agr-ctr;hasContractualElement"/>
		<rdfs:label xml:lang="en">has strike terms</rdfs:label>
		<rdfs:domain rdf:resource="&fibo-fbc-fi-fi;Option"/>
		<rdfs:range rdf:resource="&fibo-der-der-opt;OptionStrikeTerms"/>
	</owl:ObjectProperty>
	
	<owl:ObjectProperty rdf:about="&fibo-der-der-opt;includesSpecificationTerm">
		<rdfs:label xml:lang="en">includes specification term</rdfs:label>
		<rdfs:domain rdf:resource="&fibo-der-der-opt;FixedStrikeTerms"/>
		<rdfs:range rdf:resource="&fibo-der-der-opt;StrikePrice"/>
	</owl:ObjectProperty>
	
	<owl:ObjectProperty rdf:about="&fibo-der-der-opt;isOf">
		<rdfs:label xml:lang="en">is of</rdfs:label>
		<rdfs:domain rdf:resource="&fibo-der-der-opt;ObservableBestValue"/>
		<rdfs:range rdf:resource="&fibo-der-der-opt;LookbackStrikeObservable"/>
	</owl:ObjectProperty>
	
	<owl:ObjectProperty rdf:about="&fibo-der-der-opt;lookbackPeriod">
		<rdfs:label xml:lang="en">lookback period</rdfs:label>
		<rdfs:domain rdf:resource="&fibo-der-der-opt;LookbackStrikeTerms"/>
		<rdfs:range rdf:resource="&fibo-fnd-dt-fd;DatePeriod"/>
		<skos:definition xml:lang="en">The period in which the strike</skos:definition>
	</owl:ObjectProperty>
	
	<owl:DatatypeProperty rdf:about="&fibo-der-der-opt;openOutcry">
		<rdfs:label xml:lang="en">open outcry</rdfs:label>
		<rdfs:domain rdf:resource="&fibo-der-drc-bsc;DesignatedContractMarket"/>
		<rdfs:range rdf:resource="&xsd;boolean"/>
		<skos:definition xml:lang="en">Whether trading on the exchange is by way of open outcry in the form of physical interaction between participants. No means that trading is carried out electronically.</skos:definition>
	</owl:DatatypeProperty>
	
	<owl:ObjectProperty rdf:about="&fibo-der-der-opt;receives">
		<rdfs:label xml:lang="en">receives</rdfs:label>
		<rdfs:range rdf:resource="&fibo-fnd-agr-ctr;ContractualCommitment"/>
	</owl:ObjectProperty>
	
	<owl:ObjectProperty rdf:about="&fibo-der-der-opt;references">
		<rdfs:label xml:lang="en">references</rdfs:label>
		<rdfs:domain rdf:resource="&fibo-der-der-opt;BetterOrWorseOfAssetsPayoutCommitment"/>
		<rdfs:range rdf:resource="&fibo-der-der-opt;PayoffAssetsList"/>
	</owl:ObjectProperty>
	
	<owl:ObjectProperty rdf:about="&fibo-der-der-opt;strikeDeterminationDate">
		<rdfs:label xml:lang="en">strike determination date</rdfs:label>
		<rdfs:domain rdf:resource="&fibo-der-der-opt;FixedStrikeTerms"/>
		<rdfs:range rdf:resource="&fibo-fnd-dt-fd;Date"/>
		<skos:definition xml:lang="en">The date on which the strike is determined,</skos:definition>
	</owl:ObjectProperty>
	
	<owl:DatatypeProperty rdf:about="&fibo-der-der-opt;threshold">
		<rdfs:label xml:lang="en">threshold</rdfs:label>
		<rdfs:domain rdf:resource="&fibo-der-der-opt;OptionBarrierFeatureEvent"/>
		<rdfs:range rdf:resource="&xsd;decimal"/>
		<skos:definition xml:lang="en">The price or other variable (as a number) which has to be met for the event to be deemed to have occurred.</skos:definition>
	</owl:DatatypeProperty>
	
	<owl:Class rdf:about="&fibo-fbc-fi-fi;Option">
		<rdfs:subClassOf>
			<owl:Restriction>
				<owl:onProperty rdf:resource="&fibo-fnd-agr-ctr;hasContractualElement"/>
				<owl:onClass rdf:resource="&fibo-der-der-opt;OptionBarrierFeatureTerms"/>
				<owl:maxQualifiedCardinality rdf:datatype="&xsd;nonNegativeInteger">2</owl:maxQualifiedCardinality>
			</owl:Restriction>
		</rdfs:subClassOf>
		<rdfs:subClassOf>
			<owl:Restriction>
				<owl:onProperty rdf:resource="&fibo-der-der-opt;hasExercisePrice"/>
				<owl:someValuesFrom rdf:resource="&fibo-fnd-acc-cur;MonetaryPrice"/>
			</owl:Restriction>
		</rdfs:subClassOf>
		<rdfs:subClassOf>
			<owl:Restriction>
				<owl:onProperty rdf:resource="&fibo-der-der-opt;hasPremium"/>
				<owl:someValuesFrom rdf:resource="&fibo-der-der-opt;OptionPremium"/>
			</owl:Restriction>
		</rdfs:subClassOf>
		<rdfs:subClassOf>
			<owl:Restriction>
				<owl:onProperty rdf:resource="&fibo-der-der-opt;hasStrikeTerms"/>
				<owl:someValuesFrom rdf:resource="&fibo-der-der-opt;OptionStrikeTerms"/>
			</owl:Restriction>
		</rdfs:subClassOf>
		<rdfs:subClassOf>
			<owl:Restriction>
				<owl:onProperty rdf:resource="&fibo-fnd-pas-pas;hasBuyer"/>
				<owl:someValuesFrom rdf:resource="&fibo-fnd-pas-pas;Buyer"/>
			</owl:Restriction>
		</rdfs:subClassOf>
		<rdfs:subClassOf>
			<owl:Restriction>
				<owl:onProperty rdf:resource="&fibo-fnd-pas-pas;hasSeller"/>
				<owl:someValuesFrom rdf:resource="&fibo-fnd-pas-pas;Seller"/>
			</owl:Restriction>
		</rdfs:subClassOf>
		<rdfs:subClassOf>
			<owl:Restriction>
				<owl:onProperty rdf:resource="&fibo-sec-dbt-ex;hasExerciseTerms"/>
				<owl:someValuesFrom rdf:resource="&fibo-sec-dbt-ex;ExerciseTerms"/>
			</owl:Restriction>
		</rdfs:subClassOf>
	</owl:Class>

</rdf:RDF>