<?xml version="1.0" encoding="UTF-8"?>
<!DOCTYPE rdf:RDF [
	<!ENTITY dct "http://purl.org/dc/terms/">
	<!ENTITY fibo-der-der-opt "https://spec.edmcouncil.org/fibo/ontology/DER/DerivativesContracts/Options/">
	<!ENTITY fibo-der-der-sp "https://spec.edmcouncil.org/fibo/ontology/DER/DerivativesContracts/Spots/">
	<!ENTITY fibo-der-drc-bsc "https://spec.edmcouncil.org/fibo/ontology/DER/DerivativesContracts/DerivativesBasics/">
	<!ENTITY fibo-fbc-fi-fi "https://spec.edmcouncil.org/fibo/ontology/FBC/FinancialInstruments/FinancialInstruments/">
	<!ENTITY fibo-fbc-fi-stl "https://spec.edmcouncil.org/fibo/ontology/FBC/FinancialInstruments/Settlement/">
	<!ENTITY fibo-fbc-pas-fpas "https://spec.edmcouncil.org/fibo/ontology/FBC/ProductsAndServices/FinancialProductsAndServices/">
	<!ENTITY fibo-fnd-acc-cur "https://spec.edmcouncil.org/fibo/ontology/FND/Accounting/CurrencyAmount/">
	<!ENTITY fibo-fnd-agr-ctr "https://spec.edmcouncil.org/fibo/ontology/FND/Agreements/Contracts/">
	<!ENTITY fibo-fnd-pas-psch "https://spec.edmcouncil.org/fibo/ontology/FND/ProductsAndServices/PaymentsAndSchedules/">
	<!ENTITY fibo-fnd-txn-rea "https://spec.edmcouncil.org/fibo/ontology/FND/TransactionsExt/REATransactions/">
	<!ENTITY fibo-fnd-utl-av "https://spec.edmcouncil.org/fibo/ontology/FND/Utilities/AnnotationVocabulary/">
	<!ENTITY owl "http://www.w3.org/2002/07/owl#">
	<!ENTITY rdf "http://www.w3.org/1999/02/22-rdf-syntax-ns#">
	<!ENTITY rdfs "http://www.w3.org/2000/01/rdf-schema#">
	<!ENTITY skos "http://www.w3.org/2004/02/skos/core#">
	<!ENTITY sm "http://www.omg.org/techprocess/ab/SpecificationMetadata/">
	<!ENTITY xsd "http://www.w3.org/2001/XMLSchema#">
]>
<rdf:RDF xml:base="https://spec.edmcouncil.org/fibo/ontology/DER/DerivativesContracts/Spots/"
	xmlns:dct="http://purl.org/dc/terms/"
	xmlns:fibo-der-der-opt="https://spec.edmcouncil.org/fibo/ontology/DER/DerivativesContracts/Options/"
	xmlns:fibo-der-der-sp="https://spec.edmcouncil.org/fibo/ontology/DER/DerivativesContracts/Spots/"
	xmlns:fibo-der-drc-bsc="https://spec.edmcouncil.org/fibo/ontology/DER/DerivativesContracts/DerivativesBasics/"
	xmlns:fibo-fbc-fi-fi="https://spec.edmcouncil.org/fibo/ontology/FBC/FinancialInstruments/FinancialInstruments/"
	xmlns:fibo-fbc-fi-stl="https://spec.edmcouncil.org/fibo/ontology/FBC/FinancialInstruments/Settlement/"
	xmlns:fibo-fbc-pas-fpas="https://spec.edmcouncil.org/fibo/ontology/FBC/ProductsAndServices/FinancialProductsAndServices/"
	xmlns:fibo-fnd-acc-cur="https://spec.edmcouncil.org/fibo/ontology/FND/Accounting/CurrencyAmount/"
	xmlns:fibo-fnd-agr-ctr="https://spec.edmcouncil.org/fibo/ontology/FND/Agreements/Contracts/"
	xmlns:fibo-fnd-pas-psch="https://spec.edmcouncil.org/fibo/ontology/FND/ProductsAndServices/PaymentsAndSchedules/"
	xmlns:fibo-fnd-txn-rea="https://spec.edmcouncil.org/fibo/ontology/FND/TransactionsExt/REATransactions/"
	xmlns:fibo-fnd-utl-av="https://spec.edmcouncil.org/fibo/ontology/FND/Utilities/AnnotationVocabulary/"
	xmlns:owl="http://www.w3.org/2002/07/owl#"
	xmlns:rdf="http://www.w3.org/1999/02/22-rdf-syntax-ns#"
	xmlns:rdfs="http://www.w3.org/2000/01/rdf-schema#"
	xmlns:skos="http://www.w3.org/2004/02/skos/core#"
	xmlns:sm="http://www.omg.org/techprocess/ab/SpecificationMetadata/"
	xmlns:xsd="http://www.w3.org/2001/XMLSchema#">
	
	<owl:Ontology rdf:about="https://spec.edmcouncil.org/fibo/ontology/DER/DerivativesContracts/Spots/">
		<rdfs:label xml:lang="en">Spots</rdfs:label>
		<dct:abstract>Spot transactions, along with their corresponding or implied contracts. These are not a derivative but rather define simple transactions that are immediately settled by both sides, for a given kind of asset or commodity. These are the concepts common to other variants of spot such as commodities spots.</dct:abstract>
		<dct:license rdf:datatype="&xsd;anyURI">http://opensource.org/licenses/MIT</dct:license>
		<sm:contentLanguage rdf:resource="https://www.w3.org/TR/owl2-quick-reference/"/>
		<sm:copyright>Copyright (c) 2015-2021 EDM Council, Inc.</sm:copyright>
		<sm:fileAbbreviation>fibo-der-der-sp</sm:fileAbbreviation>
		<owl:imports rdf:resource="https://spec.edmcouncil.org/fibo/ontology/DER/DerivativesContracts/DerivativesBasics/"/>
		<owl:imports rdf:resource="https://spec.edmcouncil.org/fibo/ontology/DER/DerivativesContracts/Options/"/>
		<owl:imports rdf:resource="https://spec.edmcouncil.org/fibo/ontology/FBC/FinancialInstruments/FinancialInstruments/"/>
		<owl:imports rdf:resource="https://spec.edmcouncil.org/fibo/ontology/FBC/FinancialInstruments/Settlement/"/>
		<owl:imports rdf:resource="https://spec.edmcouncil.org/fibo/ontology/FBC/ProductsAndServices/FinancialProductsAndServices/"/>
		<owl:imports rdf:resource="https://spec.edmcouncil.org/fibo/ontology/FND/Accounting/CurrencyAmount/"/>
		<owl:imports rdf:resource="https://spec.edmcouncil.org/fibo/ontology/FND/Agreements/Contracts/"/>
		<owl:imports rdf:resource="https://spec.edmcouncil.org/fibo/ontology/FND/ProductsAndServices/PaymentsAndSchedules/"/>
		<owl:imports rdf:resource="https://spec.edmcouncil.org/fibo/ontology/FND/TransactionsExt/EconomicResources/"/>
		<owl:imports rdf:resource="https://spec.edmcouncil.org/fibo/ontology/FND/TransactionsExt/REATransactions/"/>
		<owl:imports rdf:resource="https://spec.edmcouncil.org/fibo/ontology/FND/Utilities/AnnotationVocabulary/"/>
		<owl:versionIRI rdf:resource="https://spec.edmcouncil.org/fibo/ontology/DER/DerivativesContracts/Spots/"/>
		<fibo-fnd-utl-av:hasMaturityLevel rdf:resource="&fibo-fnd-utl-av;Provisional"/>
	</owl:Ontology>
	
	<owl:Class rdf:about="&fibo-der-der-sp;SpotCashSettlementTerms">
		<rdfs:subClassOf rdf:resource="&fibo-fbc-fi-stl;CashSettlementTerms"/>
		<rdfs:subClassOf>
			<owl:Restriction>
				<owl:onProperty rdf:resource="&fibo-der-der-opt;hasPayer"/>
				<owl:someValuesFrom rdf:resource="&fibo-der-drc-bsc;PayingParty"/>
			</owl:Restriction>
		</rdfs:subClassOf>
		<rdfs:subClassOf>
			<owl:Restriction>
				<owl:onProperty rdf:resource="&fibo-der-der-opt;hasReceiver"/>
				<owl:someValuesFrom rdf:resource="&fibo-der-drc-bsc;ReceivingParty"/>
			</owl:Restriction>
		</rdfs:subClassOf>
		<rdfs:label xml:lang="en">spot cash settlement terms</rdfs:label>
	</owl:Class>
	
	<owl:Class rdf:about="&fibo-der-der-sp;SpotContract">
		<rdfs:subClassOf rdf:resource="&fibo-fbc-fi-fi;FinancialInstrument"/>
		<rdfs:subClassOf>
			<owl:Restriction>
				<owl:onProperty rdf:resource="&fibo-fnd-agr-ctr;hasContractualElement"/>
				<owl:someValuesFrom rdf:resource="&fibo-der-der-sp;SpotCashSettlementTerms"/>
			</owl:Restriction>
		</rdfs:subClassOf>
		<rdfs:label xml:lang="en">spot contract</rdfs:label>
		<skos:definition xml:lang="en">contract relating to a transaction which is for immediate settlement. Further notes: A spot transaction simply means a transaction in which some goods or currency are exchanged for some other goods or currency, with no future delivery provision. A Spot contract is the usually unwritten contract which by definition underlies that kind of transaction. Spot means for immediate settlement. Immediate here means the minimum number of days that are possible. This includes general retail transactions as well as the specialixed types of spot transactiojn foud in the financial services and treasury trading contexts, such as Fx Spots (a sub type of this) and commodity spot transactions. However the settlement date is still some time in the future. Also given different time zones, the settlement would be at some time in the future anyway Formerly a financial e.g. currency Spot would have been 2 (working) days settlement for example. Canadian v USD would be 1 day. Follows a settlement convention from the relevant market. Action: Add reference to Settlement Convention for the given market.</skos:definition>
	</owl:Class>
	
	<owl:Class rdf:about="&fibo-der-der-sp;SpotTransaction">
		<rdfs:subClassOf rdf:resource="&fibo-fnd-txn-rea;ContractualTransaction"/>
		<rdfs:subClassOf>
			<owl:Restriction>
				<owl:onProperty rdf:resource="&fibo-der-der-sp;hasImpliedContract"/>
				<owl:someValuesFrom rdf:resource="&fibo-der-der-sp;SpotContract"/>
			</owl:Restriction>
		</rdfs:subClassOf>
		<rdfs:subClassOf>
			<owl:Restriction>
				<owl:onProperty rdf:resource="&fibo-fnd-txn-rea;subject"/>
				<owl:someValuesFrom rdf:resource="&fibo-fnd-acc-cur;AmountOfMoney"/>
			</owl:Restriction>
		</rdfs:subClassOf>
		<rdfs:label xml:lang="en">spot transaction</rdfs:label>
	</owl:Class>
	
	<owl:ObjectProperty rdf:about="&fibo-der-der-sp;hasImpliedContract">
		<rdfs:subPropertyOf rdf:resource="&fibo-fnd-txn-rea;transactionEmbodiesEconomicAgreement"/>
		<rdfs:label xml:lang="en">has implied contract</rdfs:label>
		<rdfs:domain rdf:resource="&fibo-der-der-sp;SpotTransaction"/>
		<rdfs:range rdf:resource="&fibo-der-der-sp;SpotContract"/>
	</owl:ObjectProperty>
	
	<owl:DatatypeProperty rdf:about="&fibo-der-der-sp;paymentType">
		<rdfs:label xml:lang="en">payment type</rdfs:label>
		<rdfs:domain rdf:resource="&fibo-der-der-sp;SpotCashSettlementTerms"/>
		<rdfs:range rdf:resource="&xsd;string"/>
		<skos:definition xml:lang="en">FpML = paymentType &apos;A classification of the type of fee or additional payment, e.g. brokerage, upfront fee etc. FpML does not define domain values for this element.&apos;</skos:definition>
	</owl:DatatypeProperty>
	
	<owl:DatatypeProperty rdf:about="&fibo-der-der-sp;settlementInformation">
		<rdfs:label xml:lang="en">settlement information</rdfs:label>
		<rdfs:domain rdf:resource="&fibo-der-der-sp;SpotCashSettlementTerms"/>
		<rdfs:range rdf:resource="&xsd;string"/>
		<skos:definition xml:lang="en">FpML settlementInformation (in payment) &apos;The information required to settle a currency payment that results from a trade.&apos;</skos:definition>
	</owl:DatatypeProperty>

</rdf:RDF>