<?xml version="1.0" encoding="UTF-8"?>
<!DOCTYPE rdf:RDF [
	<!ENTITY dct "http://purl.org/dc/terms/">
	<!ENTITY fibo-der-der-sp "https://spec.edmcouncil.org/fibo/ontology/DER/DerivativesContracts/Spots/">
	<!ENTITY fibo-der-drc-bsc "https://spec.edmcouncil.org/fibo/ontology/DER/DerivativesContracts/DerivativesBasics/">
	<!ENTITY fibo-der-drc-fwd "https://spec.edmcouncil.org/fibo/ontology/DER/DerivativesContracts/Forwards/">
	<!ENTITY fibo-der-drc-swp "https://spec.edmcouncil.org/fibo/ontology/DER/DerivativesContracts/Swaps/">
	<!ENTITY fibo-der-fx-ctr "https://spec.edmcouncil.org/fibo/ontology/DER/FxDerivatives/FxContracts/">
	<!ENTITY fibo-der-rtd-rtd "https://spec.edmcouncil.org/fibo/ontology/DER/RateDerivatives/RateDerivatives/">
	<!ENTITY fibo-fbc-fi-fi "https://spec.edmcouncil.org/fibo/ontology/FBC/FinancialInstruments/FinancialInstruments/">
	<!ENTITY fibo-fbc-pas-fpas "https://spec.edmcouncil.org/fibo/ontology/FBC/ProductsAndServices/FinancialProductsAndServices/">
	<!ENTITY fibo-fnd-acc-cur "https://spec.edmcouncil.org/fibo/ontology/FND/Accounting/CurrencyAmount/">
	<!ENTITY fibo-fnd-agr-ctr "https://spec.edmcouncil.org/fibo/ontology/FND/Agreements/Contracts/">
	<!ENTITY fibo-fnd-qt-qtu "https://spec.edmcouncil.org/fibo/ontology/FND/Quantities/QuantitiesAndUnits/">
	<!ENTITY fibo-fnd-rel-rel "https://spec.edmcouncil.org/fibo/ontology/FND/Relations/Relations/">
	<!ENTITY fibo-fnd-utl-alx "https://spec.edmcouncil.org/fibo/ontology/FND/Utilities/Analytics/">
	<!ENTITY fibo-fnd-utl-av "https://spec.edmcouncil.org/fibo/ontology/FND/Utilities/AnnotationVocabulary/">
	<!ENTITY fibo-ind-fx-fx "https://spec.edmcouncil.org/fibo/ontology/IND/ForeignExchange/ForeignExchange/">
	<!ENTITY lcc-cr "https://www.omg.org/spec/LCC/Countries/CountryRepresentation/">
	<!ENTITY owl "http://www.w3.org/2002/07/owl#">
	<!ENTITY rdf "http://www.w3.org/1999/02/22-rdf-syntax-ns#">
	<!ENTITY rdfs "http://www.w3.org/2000/01/rdf-schema#">
	<!ENTITY skos "http://www.w3.org/2004/02/skos/core#">
	<!ENTITY sm "http://www.omg.org/techprocess/ab/SpecificationMetadata/">
	<!ENTITY xsd "http://www.w3.org/2001/XMLSchema#">
]>
<rdf:RDF xml:base="https://spec.edmcouncil.org/fibo/ontology/DER/FxDerivatives/FxContracts/"
	xmlns:dct="http://purl.org/dc/terms/"
	xmlns:fibo-der-der-sp="https://spec.edmcouncil.org/fibo/ontology/DER/DerivativesContracts/Spots/"
	xmlns:fibo-der-drc-bsc="https://spec.edmcouncil.org/fibo/ontology/DER/DerivativesContracts/DerivativesBasics/"
	xmlns:fibo-der-drc-fwd="https://spec.edmcouncil.org/fibo/ontology/DER/DerivativesContracts/Forwards/"
	xmlns:fibo-der-drc-swp="https://spec.edmcouncil.org/fibo/ontology/DER/DerivativesContracts/Swaps/"
	xmlns:fibo-der-fx-ctr="https://spec.edmcouncil.org/fibo/ontology/DER/FxDerivatives/FxContracts/"
	xmlns:fibo-der-rtd-rtd="https://spec.edmcouncil.org/fibo/ontology/DER/RateDerivatives/RateDerivatives/"
	xmlns:fibo-fbc-fi-fi="https://spec.edmcouncil.org/fibo/ontology/FBC/FinancialInstruments/FinancialInstruments/"
	xmlns:fibo-fbc-pas-fpas="https://spec.edmcouncil.org/fibo/ontology/FBC/ProductsAndServices/FinancialProductsAndServices/"
	xmlns:fibo-fnd-acc-cur="https://spec.edmcouncil.org/fibo/ontology/FND/Accounting/CurrencyAmount/"
	xmlns:fibo-fnd-agr-ctr="https://spec.edmcouncil.org/fibo/ontology/FND/Agreements/Contracts/"
	xmlns:fibo-fnd-qt-qtu="https://spec.edmcouncil.org/fibo/ontology/FND/Quantities/QuantitiesAndUnits/"
	xmlns:fibo-fnd-rel-rel="https://spec.edmcouncil.org/fibo/ontology/FND/Relations/Relations/"
	xmlns:fibo-fnd-utl-alx="https://spec.edmcouncil.org/fibo/ontology/FND/Utilities/Analytics/"
	xmlns:fibo-fnd-utl-av="https://spec.edmcouncil.org/fibo/ontology/FND/Utilities/AnnotationVocabulary/"
	xmlns:fibo-ind-fx-fx="https://spec.edmcouncil.org/fibo/ontology/IND/ForeignExchange/ForeignExchange/"
	xmlns:lcc-cr="https://www.omg.org/spec/LCC/Countries/CountryRepresentation/"
	xmlns:owl="http://www.w3.org/2002/07/owl#"
	xmlns:rdf="http://www.w3.org/1999/02/22-rdf-syntax-ns#"
	xmlns:rdfs="http://www.w3.org/2000/01/rdf-schema#"
	xmlns:skos="http://www.w3.org/2004/02/skos/core#"
	xmlns:sm="http://www.omg.org/techprocess/ab/SpecificationMetadata/"
	xmlns:xsd="http://www.w3.org/2001/XMLSchema#">
	
	<owl:Ontology rdf:about="https://spec.edmcouncil.org/fibo/ontology/DER/FxDerivatives/FxContracts/">
		<rdfs:label xml:lang="en">FxContracts</rdfs:label>
		<dct:abstract>Concepts common to foreign exchange derivatives (spots, forwards, options and swaps).</dct:abstract>
		<sm:fileAbbreviation>fibo-der-fx-ctr</sm:fileAbbreviation>
		<owl:imports rdf:resource="https://spec.edmcouncil.org/fibo/ontology/DER/DerivativesContracts/DerivativesBasics/"/>
		<owl:imports rdf:resource="https://spec.edmcouncil.org/fibo/ontology/DER/DerivativesContracts/Forwards/"/>
		<owl:imports rdf:resource="https://spec.edmcouncil.org/fibo/ontology/DER/DerivativesContracts/Spots/"/>
		<owl:imports rdf:resource="https://spec.edmcouncil.org/fibo/ontology/DER/DerivativesContracts/Swaps/"/>
		<owl:imports rdf:resource="https://spec.edmcouncil.org/fibo/ontology/DER/RateDerivatives/RateDerivatives/"/>
		<owl:imports rdf:resource="https://spec.edmcouncil.org/fibo/ontology/FBC/FinancialInstruments/FinancialInstruments/"/>
		<owl:imports rdf:resource="https://spec.edmcouncil.org/fibo/ontology/FBC/ProductsAndServices/FinancialProductsAndServices/"/>
		<owl:imports rdf:resource="https://spec.edmcouncil.org/fibo/ontology/FND/Accounting/CurrencyAmount/"/>
		<owl:imports rdf:resource="https://spec.edmcouncil.org/fibo/ontology/FND/Agreements/Contracts/"/>
		<owl:imports rdf:resource="https://spec.edmcouncil.org/fibo/ontology/FND/Quantities/QuantitiesAndUnits/"/>
		<owl:imports rdf:resource="https://spec.edmcouncil.org/fibo/ontology/FND/Relations/Relations/"/>
		<owl:imports rdf:resource="https://spec.edmcouncil.org/fibo/ontology/FND/Utilities/Analytics/"/>
		<owl:imports rdf:resource="https://spec.edmcouncil.org/fibo/ontology/FND/Utilities/AnnotationVocabulary/"/>
		<owl:imports rdf:resource="https://spec.edmcouncil.org/fibo/ontology/IND/ForeignExchange/ForeignExchange/"/>
		<owl:imports rdf:resource="https://www.omg.org/spec/LCC/Countries/CountryRepresentation/"/>
		<owl:versionIRI rdf:resource="https://spec.edmcouncil.org/fibo/ontology/DER/FxDerivatives/FxContracts/"/>
		<fibo-fnd-utl-av:hasMaturityLevel rdf:resource="&fibo-fnd-utl-av;Provisional"/>
	</owl:Ontology>
	
	<owl:Class rdf:about="&fibo-der-fx-ctr;ForeignExchangeDerivative">
		<rdfs:subClassOf rdf:resource="&fibo-der-rtd-rtd;RateBasedDerivativeInstrument"/>
		<rdfs:subClassOf>
			<owl:Restriction>
				<owl:onProperty rdf:resource="&fibo-der-drc-bsc;hasUnderlier"/>
				<owl:someValuesFrom rdf:resource="&fibo-der-rtd-rtd;ForeignExchangeRateObservable"/>
			</owl:Restriction>
		</rdfs:subClassOf>
		<rdfs:label xml:lang="en">foreign exchange derivative</rdfs:label>
		<fibo-fnd-utl-av:abbreviation xml:lang="en">FX derivative</fibo-fnd-utl-av:abbreviation>
		<fibo-fnd-utl-av:synonym xml:lang="en">forex derivative</fibo-fnd-utl-av:synonym>
	</owl:Class>
	
	<owl:Class rdf:about="&fibo-der-fx-ctr;ForeignExchangeForward">
		<rdfs:subClassOf rdf:resource="&fibo-der-drc-fwd;Forward"/>
		<rdfs:subClassOf rdf:resource="&fibo-der-fx-ctr;ForeignExchangeDerivative"/>
		<rdfs:label xml:lang="en">foreign exchange forward</rdfs:label>
		<skos:definition xml:lang="en">agreement to deliver and settle a given amount of currency in one currency, in exchange for a given amount in another currency, at an agreed date in the future and at an agreed rate of exchange</skos:definition>
	</owl:Class>
	
	<owl:Class rdf:about="&fibo-der-fx-ctr;ForeignExchangeForwardOutright">
		<rdfs:subClassOf rdf:resource="&fibo-der-fx-ctr;ForeignExchangeForward"/>
		<rdfs:subClassOf>
			<owl:Restriction>
				<owl:onProperty rdf:resource="&lcc-cr;hasPart"/>
				<owl:someValuesFrom rdf:resource="&fibo-der-fx-ctr;ForeignExchangeSpotContract"/>
			</owl:Restriction>
		</rdfs:subClassOf>
		<rdfs:subClassOf>
			<owl:Restriction>
				<owl:onProperty rdf:resource="&lcc-cr;hasPart"/>
				<owl:someValuesFrom rdf:resource="&fibo-der-fx-ctr;ForeignExchangeSwap"/>
			</owl:Restriction>
		</rdfs:subClassOf>
		<rdfs:label xml:lang="en">foreign exchange forward outright</rdfs:label>
		<skos:definition xml:lang="en">forward contract in the forex market that locks in the price at which an entity can buy or sell a currency on a future date. Also known as &quot;outright forward currency transaction&quot;, &quot;forward outright&quot; or &quot;FX forward&quot;.</skos:definition>
		<fibo-fnd-utl-av:explanatoryNote xml:lang="en">In currency forward contracts, the contract holders are obligated to buy or sell the currency at a specified price, at a specified quantity and on a specified future date. These contracts cannot be transferred. Jan 10 Review Notes Outright Forward is the term for the professional markets. Spot + Swap where Swap is 2 simultaneous transactions.</fibo-fnd-utl-av:explanatoryNote>
	</owl:Class>
	
	<owl:Class rdf:about="&fibo-der-fx-ctr;ForeignExchangeSpotContract">
		<rdfs:subClassOf rdf:resource="&fibo-der-der-sp;SpotContract"/>
		<rdfs:subClassOf rdf:resource="&fibo-der-fx-ctr;ForeignExchangeDerivative"/>
		<rdfs:label xml:lang="en">foreign exchange spot contract</rdfs:label>
		<skos:definition xml:lang="en">The rate of a foreign-exchange contract for immediate delivery. Also known as &quot;benchmark rates&quot;, &quot;straightforward rates&quot; or &quot;outright rates&quot;, spot rates represent the price that a buyer expects to pay for a foreign currency in another currency.</skos:definition>
		<fibo-fnd-utl-av:explanatoryNote xml:lang="en">Though the spot exchange rate is said to be settled immediately, the globally accepted settlement cycle for foreign-exchange contracts is two days. Foreign-exchange contracts are therefore settled on the second day after the day the deal is made.</fibo-fnd-utl-av:explanatoryNote>
	</owl:Class>
	
	<owl:Class rdf:about="&fibo-der-fx-ctr;ForeignExchangeSwap">
		<rdfs:subClassOf rdf:resource="&fibo-der-drc-swp;Swap"/>
		<rdfs:subClassOf rdf:resource="&fibo-der-fx-ctr;ForeignExchangeDerivative"/>
		<rdfs:subClassOf>
			<owl:Restriction>
				<owl:onProperty rdf:resource="&fibo-der-drc-swp;hasLeg"/>
				<owl:someValuesFrom rdf:resource="&fibo-der-fx-ctr;ForeignExchangeForward"/>
			</owl:Restriction>
		</rdfs:subClassOf>
		<rdfs:subClassOf>
			<owl:Restriction>
				<owl:onProperty rdf:resource="&fibo-der-drc-swp;hasLeg"/>
				<owl:someValuesFrom rdf:resource="&fibo-der-fx-ctr;ForeignExchangeSpotContract"/>
			</owl:Restriction>
		</rdfs:subClassOf>
		<rdfs:label xml:lang="en">foreign exchange swap</rdfs:label>
	</owl:Class>
	
	<owl:ObjectProperty rdf:about="&fibo-der-fx-ctr;hasBuyerCurrency">
		<rdfs:subPropertyOf rdf:resource="&fibo-fnd-acc-cur;hasDealtCurrency"/>
		<rdfs:label xml:lang="en">has buyer currency</rdfs:label>
		<rdfs:domain rdf:resource="&fibo-der-fx-ctr;ForeignExchangeSpotContract"/>
		<rdfs:range rdf:resource="&fibo-fnd-acc-cur;Currency"/>
		<skos:definition xml:lang="en">The buyer&apos;s currency as specified in the contract.</skos:definition>
	</owl:ObjectProperty>
	
	<owl:ObjectProperty rdf:about="&fibo-der-fx-ctr;hasExchangedCurrencyOne">
		<rdfs:subPropertyOf rdf:resource="&fibo-fnd-acc-cur;hasCurrency"/>
		<rdfs:label xml:lang="en">has exchanged currency one</rdfs:label>
		<rdfs:domain rdf:resource="&fibo-der-fx-ctr;ForeignExchangeForward"/>
		<rdfs:range rdf:resource="&fibo-fnd-acc-cur;Currency"/>
		<skos:definition xml:lang="en">FpML has a term exchangedCurrency1 but this refers to the currency flow not the currency as in USD, CDN etc. FpML definition for exchangedCurrency1: &apos;This is the first of the two currency flows that define a single leg of a standard foreign exchange transaction.&apos;</skos:definition>
	</owl:ObjectProperty>
	
	<owl:ObjectProperty rdf:about="&fibo-der-fx-ctr;hasExchangedCurrencyTwo">
		<rdfs:subPropertyOf rdf:resource="&fibo-fnd-acc-cur;hasCurrency"/>
		<rdfs:label xml:lang="en">has exchanged currency two</rdfs:label>
		<rdfs:domain rdf:resource="&fibo-der-fx-ctr;ForeignExchangeForward"/>
		<rdfs:range rdf:resource="&fibo-fnd-acc-cur;Currency"/>
	</owl:ObjectProperty>
	
	<owl:ObjectProperty rdf:about="&fibo-der-fx-ctr;hasForeignExchangeForwardRate">
		<rdfs:subPropertyOf rdf:resource="&fibo-fnd-qt-qtu;hasQuantityValue"/>
		<rdfs:label xml:lang="en">has foreign exchange forward rate</rdfs:label>
		<rdfs:domain rdf:resource="&fibo-der-fx-ctr;ForeignExchangeForwardOutright"/>
		<rdfs:range rdf:resource="&fibo-fnd-acc-cur;ExchangeRate"/>
		<skos:definition xml:lang="en">The rate at which the seller currency is purchased in the buyer currency.</skos:definition>
	</owl:ObjectProperty>
	
	<owl:DatatypeProperty rdf:about="&fibo-der-fx-ctr;hasForeignExchangeForwardRateValue">
		<rdfs:subPropertyOf rdf:resource="&fibo-fnd-acc-cur;hasRateValue"/>
		<rdfs:label xml:lang="en">has foreign exchange forward rate value</rdfs:label>
		<rdfs:domain rdf:resource="&fibo-der-fx-ctr;ForeignExchangeForward"/>
		<rdfs:range rdf:resource="&xsd;decimal"/>
		<skos:definition xml:lang="en">&apos;The rate of exchange between the two currencies.&apos;</skos:definition>
	</owl:DatatypeProperty>
	
	<owl:ObjectProperty rdf:about="&fibo-der-fx-ctr;hasForeignExchangeSpotRate">
		<rdfs:subPropertyOf rdf:resource="&fibo-fnd-qt-qtu;hasQuantityValue"/>
		<rdfs:label xml:lang="en">has foreign exchange spot rate</rdfs:label>
		<rdfs:domain rdf:resource="&fibo-der-fx-ctr;ForeignExchangeSpotContract"/>
		<rdfs:range rdf:resource="&fibo-fnd-acc-cur;ExchangeRate"/>
		<skos:definition xml:lang="en">The rate at which the seller currency is purchased in the buyer currency.</skos:definition>
	</owl:ObjectProperty>
	
	<owl:DatatypeProperty rdf:about="&fibo-der-fx-ctr;hasForeignExchangeSpotRateValue">
		<rdfs:subPropertyOf rdf:resource="&fibo-fnd-acc-cur;hasRateValue"/>
		<rdfs:label xml:lang="en">has foreign exchange spot rate</rdfs:label>
		<rdfs:domain rdf:resource="&fibo-der-fx-ctr;ForeignExchangeSpotContract"/>
		<rdfs:range rdf:resource="&xsd;decimal"/>
		<skos:definition xml:lang="en">&apos;The rate of exchange between the two currencies.&apos;</skos:definition>
	</owl:DatatypeProperty>
	
	<owl:ObjectProperty rdf:about="&fibo-der-fx-ctr;hasSellerCurrency">
		<rdfs:subPropertyOf rdf:resource="&fibo-fnd-acc-cur;hasBaseCurrency"/>
		<rdfs:label xml:lang="en">has seller currency</rdfs:label>
		<rdfs:domain rdf:resource="&fibo-der-fx-ctr;ForeignExchangeSpotContract"/>
		<rdfs:range rdf:resource="&fibo-fnd-acc-cur;Currency"/>
		<skos:definition xml:lang="en">The seller&apos;s currency as specified in the contract.</skos:definition>
	</owl:ObjectProperty>

</rdf:RDF>